## 문제 5
함수 $f(x) = 2x^2 + ax$에 대하여 
$
\lim_{h \to 0} \frac{f(1+h) - f(1)}{h} = 6
$
일 때, 상수 $a$의 값은? **[3점]**

1. $-4$
2. $-2$
3. $0$
4. $2$
5. $4$

### 해설

함수 $f(x)$의 미분계수는 다음과 같이 주어집니다:

$
f'(x) = \lim_{h \to 0} \frac{f(x+h) - f(x)}{h}
$

주어진 함수 $f(x) = 2x^2 + ax$에서 $f(1)$과 $f(1+h)$를 계산합니다:

$
f(1) = 2(1)^2 + a(1) = 2 + a
$
$
f(1+h) = 2(1+h)^2 + a(1+h) = 2(1 + 2h + h^2) + a + ah = 2 + 4h + 2h^2 + a + ah
$

따라서 다음을 얻습니다:

$
\frac{f(1+h) - f(1)}{h} = \frac{(2 + 4h + 2h^2 + a + ah) - (2 + a)}{h} = \frac{4h + 2h^2 + ah}{h} = 4 + 2h + a
$

$h \to 0$일 때, $2h$는 0이 되므로:

$
\lim_{h \to 0} \frac{f(1+h) - f(1)}{h} = 4 + a
$

주어진 조건에 따르면 $4 + a = 6$이므로 $a = 2$입니다.

정답은 4번입니다.

## Question 5
Given the function $f(x) = 2x^2 + ax$, 
$
\lim_{h \to 0} \frac{f(1+h) - f(1)}{h} = 6
$
Find the value of the constant $a$. **[3 points]**

1. $-4$
2. $-2$
3. $0$
4. $2$
5. $4$

### Solution

The derivative of the function $f(x)$ is given by:

$
f'(x) = \lim_{h \to 0} \frac{f(x+h) - f(x)}{h}
$

For the given function $f(x) = 2x^2 + ax$, we calculate $f(1)$ and $f(1+h)$:

$
f(1) = 2(1)^2 + a(1) = 2 + a
$
$
f(1+h) = 2(1+h)^2 + a(1+h) = 2(1 + 2h + h^2) + a + ah = 2 + 4h + 2h^2 + a + ah
$

Therefore, we have:

$
\frac{f(1+h) - f(1)}{h} = \frac{(2 + 4h + 2h^2 + a + ah) - (2 + a)}{h} = \frac{4h + 2h^2 + ah}{h} = 4 + 2h + a
$

As $h \to 0$, $2h$ becomes 0, so:

$
\lim_{h \to 0} \frac{f(1+h) - f(1)}{h} = 4 + a
$

Given that $4 + a = 6$, we find $a = 2$.

The correct answer is choice 4.