

## 문제 27
수열 ${a_n}$에 대하여

$\sum_{k=1}^{10} (a_k+1)^2 = 28$, $\sum_{k=1}^{10} a_k(a_k+1) = 16$

일 때, $\sum_{k=1}^{10} (a_k)^2$의 값을 구하시오. **[4점]**

### 해설
주어진 조건을 이용하여 단계별로 풀어봅시다.

1. 첫 번째 조건: $\sum_{k=1}^{10} (a_k+1)^2 = 28$
   이를 전개하면: $\sum_{k=1}^{10} (a_k^2 + 2a_k + 1) = 28$

2. 두 번째 조건: $\sum_{k=1}^{10} a_k(a_k+1) = 16$
   이는 $\sum_{k=1}^{10} (a_k^2 + a_k) = 16$와 같습니다.

3. 우리가 구하고자 하는 것은 $\sum_{k=1}^{10} (a_k)^2$입니다.

4. 첫 번째 조건에서 두 번째 조건을 빼면:
   $\sum_{k=1}^{10} (a_k^2 + 2a_k + 1) - \sum_{k=1}^{10} (a_k^2 + a_k) = 28 - 16$
   $\sum_{k=1}^{10} (a_k + 1) = 12$

5. 따라서, $\sum_{k=1}^{10} a_k = 2$

6. 이제 첫 번째 조건을 다시 살펴보면:
   $\sum_{k=1}^{10} (a_k^2 + 2a_k + 1) = 28$
   $\sum_{k=1}^{10} a_k^2 + 2(\sum_{k=1}^{10} a_k) + 10 = 28$
   $\sum_{k=1}^{10} a_k^2 + 2(2) + 10 = 28$
   $\sum_{k=1}^{10} a_k^2 = 14$

따라서, $\sum_{k=1}^{10} (a_k)^2 = 14$입니다.

## Question 27
For a sequence ${a_n}$, given that

$\sum_{k=1}^{10} (a_k+1)^2 = 28$, $\sum_{k=1}^{10} a_k(a_k+1) = 16$

Find the value of $\sum_{k=1}^{10} (a_k)^2$. **[4 points]**

### Solution
Let's solve this step by step using the given conditions.

1. First condition: $\sum_{k=1}^{10} (a_k+1)^2 = 28$
   Expanding this: $\sum_{k=1}^{10} (a_k^2 + 2a_k + 1) = 28$

2. Second condition: $\sum_{k=1}^{10} a_k(a_k+1) = 16$
   This is equivalent to $\sum_{k=1}^{10} (a_k^2 + a_k) = 16$

3. We want to find $\sum_{k=1}^{10} (a_k)^2$

4. Subtracting the second condition from the first:
   $\sum_{k=1}^{10} (a_k^2 + 2a_k + 1) - \sum_{k=1}^{10} (a_k^2 + a_k) = 28 - 16$
   $\sum_{k=1}^{10} (a_k + 1) = 12$

5. Therefore, $\sum_{k=1}^{10} a_k = 2$

6. Now, looking back at the first condition:
   $\sum_{k=1}^{10} (a_k^2 + 2a_k + 1) = 28$
   $\sum_{k=1}^{10} a_k^2 + 2(\sum_{k=1}^{10} a_k) + 10 = 28$
   $\sum_{k=1}^{10} a_k^2 + 2(2) + 10 = 28$
   $\sum_{k=1}^{10} a_k^2 = 14$

Thus, $\sum_{k=1}^{10} (a_k)^2 = 14$.