

## 문제 24
$\lim \limits_{x \to \infty} \frac{1}{n} \sum_{k =1}^{n} \sqrt{1 + \frac{3k}{n}}$의 값은? **[3점]**

1. $\frac{4}{3}$  
2. $\frac{13}{9}$  
3. $\frac{14}{9}$  
4. $\frac{5}{3}$  
5. $\frac{16}{9}$

### 해설
1. **문제의 형태**:
   - 주어진 문제는 리만 합의 극한을 계산하는 문제입니다.
   - 이 형태는 리만 합의 정의를 통해 정적분의 값으로 변환될 수 있습니다.

2. **리만 합의 정의**:
   - 주어진 리만 합 $\frac{1}{n} \sum_{k=1}^{n} \sqrt{1 + \frac{3k}{n}}$은 다음과 같이 해석될 수 있습니다.
   - 함수 $f(x) = \sqrt{1 + 3x}$의 $[0,1]$ 구간에 대한 리만 합입니다.
   - 이를 식으로 표현하면:
   $$
   \lim_{n \to \infty} \frac{1}{n} \sum_{k=1}^{n} f\left(\frac{k}{n}\right) = \int_{0}^{1} \sqrt{1 + 3x} \, dx
   $$

3. **정적분 계산**:
   - $\int_{0}^{1} \sqrt{1 + 3x} \, dx$를 계산합니다.
   - $u$ 치환법을 사용하여 $u = 1 + 3x$, $du = 3dx$로 바꿉니다.
   $$
   \int_{0}^{1} \sqrt{1 + 3x} \, dx = \frac{2}{9} \left[(1 + 3x)^{3/2}\right]_{0}^{1} = \frac{2}{9} \left[(4)^{3/2} - (1)^{3/2}\right] = \frac{2}{9} \times (8 - 1) = \frac{14}{9}
   $$

정답은 **$\frac{14}{9}$**입니다.

---

## Question 24
Find the value of $\lim \limits_{x \to \infty} \frac{1}{n} \sum_{k =1}^{n} \sqrt{1 + \frac{3k}{n}}$. **[3 points]**

1. $\frac{4}{3}$  
2. $\frac{13}{9}$  
3. $\frac{14}{9}$  
4. $\frac{5}{3}$  
5. $\frac{16}{9}$

### Solution
1. **Form of the Problem**:
   - The problem involves evaluating the limit of a Riemann sum.
   - This form can be converted into the value of a definite integral using the definition of a Riemann sum.

2. **Definition of Riemann Sum**:
   - The given Riemann sum $\frac{1}{n} \sum_{k=1}^{n} \sqrt{1 + \frac{3k}{n}}$ can be interpreted as:
   - The function $f(x) = \sqrt{1 + 3x}$ over the interval $[0,1]$.
   - Expressing this as an integral:
   $$
   \lim_{n \to \infty} \frac{1}{n} \sum_{k=1}^{n} f\left(\frac{k}{n}\right) = \int_{0}^{1} \sqrt{1 + 3x} \, dx
   $$

3. **Calculating the Integral**:
   - Now, we calculate $\int_{0}^{1} \sqrt{1 + 3x} \, dx$.
   - Using the substitution $u = 1 + 3x$, $du = 3dx$, the integral becomes:
   $$
   \int_{0}^{1} \sqrt{1 + 3x} \, dx = \frac{2}{9} \left[(1 + 3x)^{3/2}\right]_{0}^{1} = \frac{2}{9} \left[(4)^{3/2} - (1)^{3/2}\right] = \frac{2}{9} \times (8 - 1) = \frac{14}{9}
   $$

The correct answer is **$\frac{14}{9}$**.

