
## 문제 29
세 상수 $a$, $b$, $c$에 대하여 함수 $f(x)=ae^{2x}+be^x+c$가 다음 조건을 만족시킨다.

(가) $\lim_{x \to -\infty} \frac{f(x)+6}{e^x} = 1$

(나) $f(\ln 2) = 0$

함수 $f(x)$의 역함수를 $g(x)$라 할 때,

$\int_0^1 g(x)dx = p+q\ln 2$이다. $p+q$의 값을 구하시오.

(단, $p$, $q$는 유리수이고, $\ln 2$는 무리수이다.) **[4점]**

### 해설

1) 조건 (가)에서 $\lim_{x \to -\infty} \frac{f(x)+6}{e^x} = 1$이므로:
   $\lim_{x \to -\infty} \frac{ae^{2x}+be^x+c+6}{e^x} = 1$
   $\lim_{x \to -\infty} (ae^x+b+\frac{c+6}{e^x}) = 1$
   따라서 $b=1$, $c=-6$

2) 조건 (나)에서 $f(\ln 2) = 0$이므로:
   $a(2)^2 + 1(2) + (-6) = 0$
   $4a + 2 - 6 = 0$
   $4a = 4$
   $a = 1$

3) 따라서 $f(x) = e^{2x} + e^x - 6$

4) $f(x)$의 역함수 $g(x)$를 구하기 위해:
   $y = e^{2x} + e^x - 6$
   $y + 6 = e^{2x} + e^x$
   $y + 6 = e^x(e^x + 1)$
   $e^x = \frac{y+6}{e^x+1}$

5) $\int_0^1 g(x)dx = p+q\ln 2$이므로:
   $\int_0^1 \ln(\frac{x+6}{x+1})dx = p+q\ln 2$

6) 적분 계산:
   $\int_0^1 \ln(x+6)dx - \int_0^1 \ln(x+1)dx$
   $= [(x+6)\ln(x+6)-x]_0^1 - [(x+1)\ln(x+1)-x]_0^1$
   $= [7\ln7-1-6\ln6] - [2\ln2-1-\ln1]$
   $= 7\ln7 - 6\ln6 - 2\ln2 + 1$

7) 따라서 $p = 1$, $q = 7\ln7 - 6\ln6 - 2\ln2 = 1$

8) $p + q = 1 + 1 = 2$

따라서 $p+q$의 값은 2입니다.

## Question 29
For three constants $a$, $b$, and $c$, the function $f(x)=ae^{2x}+be^x+c$ satisfies the following conditions:

(a) $\lim_{x \to -\infty} \frac{f(x)+6}{e^x} = 1$

(b) $f(\ln 2) = 0$

When the inverse function of $f(x)$ is $g(x)$,

$\int_0^1 g(x)dx = p+q\ln 2$. Find the value of $p+q$.

(Note: $p$ and $q$ are rational numbers, and $\ln 2$ is an irrational number.) **[4 points]**

### Solution

1) From condition (a), $\lim_{x \to -\infty} \frac{f(x)+6}{e^x} = 1$:
   $\lim_{x \to -\infty} \frac{ae^{2x}+be^x+c+6}{e^x} = 1$
   $\lim_{x \to -\infty} (ae^x+b+\frac{c+6}{e^x}) = 1$
   Therefore, $b=1$, $c=-6$

2) From condition (b), $f(\ln 2) = 0$:
   $a(2)^2 + 1(2) + (-6) = 0$
   $4a + 2 - 6 = 0$
   $4a = 4$
   $a = 1$

3) Thus, $f(x) = e^{2x} + e^x - 6$

4) To find the inverse function $g(x)$ of $f(x)$:
   $y = e^{2x} + e^x - 6$
   $y + 6 = e^{2x} + e^x$
   $y + 6 = e^x(e^x + 1)$
   $e^x = \frac{y+6}{e^x+1}$

5) Since $\int_0^1 g(x)dx = p+q\ln 2$:
   $\int_0^1 \ln(\frac{x+6}{x+1})dx = p+q\ln 2$

6) Calculate the integral:
   $\int_0^1 \ln(x+6)dx - \int_0^1 \ln(x+1)dx$
   $= [(x+6)\ln(x+6)-x]_0^1 - [(x+1)\ln(x+1)-x]_0^1$
   $= [7\ln7-1-6\ln6] - [2\ln2-1-\ln1]$
   $= 7\ln7 - 6\ln6 - 2\ln2 + 1$

7) Therefore, $p = 1$, $q = 7\ln7 - 6\ln6 - 2\ln2 = 1$

8) $p + q = 1 + 1 = 2$

Thus, the value of $p+q$ is 2.