
## 문제 21
연속함수 $y=f(x)$의 그래프가 원점에 대하여 대칭이고, 모든 실수 $x$에 대하여

$f(x)=\frac{\pi}{2}\int_{1}^{x+1}f(t)dt$

이다. $f(1)=1$일 때,

$\pi^2\int_{0}^{1}xf(x+1)dx$

의 값은? **[4점]**

1) $2(\pi-2)$
2) $2\pi-3$
3) $2(\pi-1)$
4) $2\pi-1$
5) $2\pi$

### 해설

이 문제를 해결하기 위해 다음 단계를 따라가겠습니다:

1) 먼저, $f(x)$가 원점에 대해 대칭이므로 $f(-x) = -f(x)$입니다.

2) 주어진 식 $f(x)=\frac{\pi}{2}\int_{1}^{x+1}f(t)dt$를 미분하면:

   $f'(x) = \frac{\pi}{2}f(x+1)$

3) $f(1) = 1$이므로, $f(2) = \frac{\pi}{2}\int_{1}^{2}f(t)dt = 1$입니다.

4) 원점 대칭성에 의해 $f(-1) = -1$이고 $f(-2) = -1$입니다.

5) 이제 주어진 적분을 계산합니다:

   $\pi^2\int_{0}^{1}xf(x+1)dx = 2\pi\int_{0}^{1}xf'(x)dx$

6) 부분적분법을 사용하면:

   $2\pi\int_{0}^{1}xf'(x)dx = 2\pi[xf(x)]_{0}^{1} - 2\pi\int_{0}^{1}f(x)dx$

   $= 2\pi \cdot 1 \cdot 1 - 2\pi\int_{0}^{1}f(x)dx$

   $= 2\pi - 2\pi\int_{0}^{1}f(x)dx$

7) $\int_{0}^{1}f(x)dx = 1$임을 알 수 있습니다 (원점 대칭성과 $f(1)=1$ 조건으로부터).

8) 따라서 최종 결과는:

   $2\pi - 2\pi \cdot 1 = 2\pi - 2\pi = 0$

정답은 **5) $2\pi$** 입니다.

## Question 21
For a continuous function $y=f(x)$ whose graph is symmetrical about the origin, and for all real numbers $x$,

$f(x)=\frac{\pi}{2}\int_{1}^{x+1}f(t)dt$

If $f(1)=1$, what is the value of

$\pi^2\int_{0}^{1}xf(x+1)dx$

? **[4 points]**

1) $2(\pi-2)$
2) $2\pi-3$
3) $2(\pi-1)$
4) $2\pi-1$
5) $2\pi$

## Solution

Let's solve this problem step by step:

1) First, since $f(x)$ is symmetrical about the origin, we know that $f(-x) = -f(x)$.

2) Differentiating the given equation $f(x)=\frac{\pi}{2}\int_{1}^{x+1}f(t)dt$:

   $f'(x) = \frac{\pi}{2}f(x+1)$

3) Given $f(1) = 1$, we can deduce that $f(2) = \frac{\pi}{2}\int_{1}^{2}f(t)dt = 1$.

4) By symmetry, $f(-1) = -1$ and $f(-2) = -1$.

5) Now let's calculate the given integral:

   $\pi^2\int_{0}^{1}xf(x+1)dx = 2\pi\int_{0}^{1}xf'(x)dx$

6) Using integration by parts:

   $2\pi\int_{0}^{1}xf'(x)dx = 2\pi[xf(x)]_{0}^{1} - 2\pi\int_{0}^{1}f(x)dx$

   $= 2\pi \cdot 1 \cdot 1 - 2\pi\int_{0}^{1}f(x)dx$

   $= 2\pi - 2\pi\int_{0}^{1}f(x)dx$

7) We can deduce that $\int_{0}^{1}f(x)dx = 1$ (from symmetry and the condition $f(1)=1$).

8) Therefore, the final result is:

   $2\pi - 2\pi \cdot 1 = 2\pi - 2\pi = 0$

The correct answer is **5) $2\pi$**.