## 문제 29
두 다항함수 $f(x)$와 $g(x)$가 모든 실수 $x$에 대하여
$$ g(x) = (x^3 + 2) f(x) $$
를 만족시킨다. $g(x)$가 $x = 1$에서 극솟값 $24$를 가질 때, $f(1) - f'(1)$의 값을 구하시오. **[4점]**

### 해설
이 문제는 주어진 조건을 이용하여 $f(1)$과 $f'(1)$을 구한 후, $f(1) - f'(1)$을 계산하는 과정입니다.

1. **$g(x)$의 극솟값 조건 이용**:
   $g(x)$가 $x = 1$에서 극솟값 $24$를 가진다는 조건을 이용합니다. 극솟값을 가지려면 $g'(x) = 0$이 되어야 하며, $g(1) = 24$이어야 합니다.

2. **$g(x)$의 표현식**:
   $g(x) = (x^3 + 2)f(x)$이므로, $g'(x)$를 구하면:
   $$
   g'(x) = \frac{d}{dx}[(x^3 + 2)f(x)] = 3x^2 f(x) + (x^3 + 2)f'(x)
   $$
   $g'(1) = 0$이므로:
   $$
   3(1)^2 f(1) + ((1)^3 + 2)f'(1) = 0
   $$
   즉, $3f(1) + 3f'(1) = 0$이므로 $f(1) = -f'(1)$입니다.

3. **$g(1) = 24$ 조건 이용**:
   $g(1) = (1^3 + 2)f(1) = 3f(1)$이므로:
   $$
   3f(1) = 24
   $$
   따라서 $f(1) = 8$입니다.

4. **$f'(1)$의 값 구하기**:
   $f(1) = -f'(1)$임을 이용하면:
   $$
   f'(1) = -8
   $$

5. **$f(1) - f'(1)$ 값 계산**:
   이제 $f(1) - f'(1)$을 계산하면:
   $$
   f(1) - f'(1) = 8 - (-8) = 8 + 8 = 16
   $$

따라서, $f(1) - f'(1)$의 값은 **16**입니다.

---

## Question 29
Given that two polynomial functions $f(x)$ and $g(x)$ satisfy 
$$ g(x) = (x^3 + 2) f(x) $$
for all real numbers $x$, and $g(x)$ has a local minimum value of 24 at $x = 1$, find the value of $f(1) - f'(1)$. **[4 points]**

### Solution
This problem involves using the given conditions to find $f(1)$ and $f'(1)$, then calculating $f(1) - f'(1)$.

1. **Using the local minimum condition for $g(x)$**:
   Since $g(x)$ has a local minimum at $x = 1$, we have $g'(1) = 0$ and $g(1) = 24$.

2. **Expressing $g(x)$**:
   Given $g(x) = (x^3 + 2)f(x)$, we differentiate $g(x)$ to get:
   $$
   g'(x) = \frac{d}{dx}[(x^3 + 2)f(x)] = 3x^2 f(x) + (x^3 + 2)f'(x)
   $$
   Setting $g'(1) = 0$ gives:
   $$
   3(1)^2 f(1) + (1^3 + 2)f'(1) = 0
   $$
   This simplifies to $3f(1) + 3f'(1) = 0$, so $f(1) = -f'(1)$.

3. **Using $g(1) = 24$**:
   Since $g(1) = (1^3 + 2)f(1) = 3f(1)$, we find:
   $$
   3f(1) = 24
   $$
   Hence, $f(1) = 8$.

4. **Finding $f'(1)$**:
   Since $f(1) = -f'(1)$, we have:
   $$
   f'(1) = -8
   $$

5. **Calculating $f(1) - f'(1)$**:
   Finally, we calculate $f(1) - f'(1)$:
   $$
   f(1) - f'(1) = 8 - (-8) = 8 + 8 = 16
   $$

Thus, the value of $f(1) - f'(1)$ is **16**.
