## 문제 17
등차수열 $ \{ a_n \} $ 이 $ \sum_{k = 1}^{n} a_{2k - 1} = 3n^2 + n $ 을 만족시킬 때, $ a_8 $의 값은? **[4점]**

1. 16  
2. 19  
3. 22  
4. 25  
5. 28  

### 해설  
주어진 등차수열 $ \{ a_n \} $의 합을 이용하여 $ a_8 $의 값을 구해봅시다.

1. $ a_{2k-1} $는 등차수열의 홀수 번째 항을 나타냅니다. 따라서 $ \sum_{k=1}^{n} a_{2k-1} $는 홀수 번째 항들의 합입니다.
   
2. 주어진 식에 따라 $ n $번째 홀수 항까지의 합은 $ 3n^2 + n $입니다. 이 식을 이용하여 일반항 $ a_{2k-1} $을 구할 수 있습니다.
   
3. $ n = 1 $일 때, $ a_1 = 3(1)^2 + 1 = 4 $입니다.

4. $ n = 2 $일 때,

   $
   a_1 + a_3 = 3(2)^2 + 2 = 14
   $

   따라서, $ a_3 = 14 - 4 = 10 $입니다.

5. $ n = 3 $일 때,

   $
   a_1 + a_3 + a_5 = 3(3)^2 + 3 = 30
   $

   따라서, $ a_5 = 30 - 14 = 16 $입니다.

6. $ n = 4 $일 때,

   $
   a_1 + a_3 + a_5 + a_7 = 3(4)^2 + 4 = 52
   $

   따라서, $ a_7 = 52 - 30 = 22 $입니다.

7. $ a_8 $은 짝수 번째 항이므로, 등차수열의 공차를 이용하여 $ a_2 = 7, a_4 = 13 $ 등의 값을 구한 뒤 $ a_8 $을 구할 수 있습니다.

8. 일반적으로 $ a_n = a_1 + (n-1)d $로 표현되므로, $ a_8 $은 다음과 같이 계산됩니다:

   $
   a_8 = a_7 + d = 22 + 6 = 28
   $

정답은 **5번: 28** 입니다.

## Question 17
Given the arithmetic sequence $ \{ a_n \} $ satisfying $ \sum_{k = 1}^{n} a_{2k - 1} = 3n^2 + n $, find the value of $ a_8 $. **[4 points]**

1. 16  
2. 19  
3. 22  
4. 25  
5. 28  

### Solution  
Let's find the value of $ a_8 $ using the sum of the given arithmetic sequence.

1. $ a_{2k-1} $ represents the odd-numbered terms in the sequence. Therefore, $ \sum_{k=1}^{n} a_{2k-1} $ is the sum of the odd-numbered terms.

2. The given formula tells us that the sum of the first $ n $ odd-numbered terms is $ 3n^2 + n $. We can use this to find the individual terms $ a_{2k-1} $.

3. For $ n = 1 $, we have $ a_1 = 3(1)^2 + 1 = 4 $.

4. For $ n = 2 $,

   $
   a_1 + a_3 = 3(2)^2 + 2 = 14
   $

   Therefore, $ a_3 = 14 - 4 = 10 $.

5. For $ n = 3 $,

   $
   a_1 + a_3 + a_5 = 3(3)^2 + 3 = 30
   $

   Therefore, $ a_5 = 30 - 14 = 16 $.

6. For $ n = 4 $,

   $
   a_1 + a_3 + a_5 + a_7 = 3(4)^2 + 4 = 52
   $
   Therefore, $ a_7 = 52 - 30 = 22 $.

7. $ a_8 $ is an even-numbered term, so we can find it using the common difference $ d $ of the sequence and previous terms like $ a_2 = 7 $ and $ a_4 = 13 $.

8. Since $ a_n = a_1 + (n-1)d $, we calculate $ a_8 $ as:

   $
   a_8 = a_7 + d = 22 + 6 = 28
   $

The correct answer is **5: 28**.
