

## 문제 9
실수 전체의 집합에서 미분가능한 함수 $f(x)$에 대하여 함수 $g(x)$를

$g(x) = \frac{f(x)}{e^{x-2}}$

라 하자. $\lim_{x \to 2} \frac{f(x)-3}{x-2} = 5$일 때, $g'(2)$의 값은? **[3점]**

1. 1
2. 2
3. 3
4. 4
5. 5

### 해설

1) 먼저 $g(x)$의 도함수를 구합니다.

   $g'(x) = \frac{f'(x)e^{x-2} - f(x)e^{x-2}}{(e^{x-2})^2}$
   
   $= \frac{f'(x)e^{x-2} - f(x)e^{x-2}}{e^{2x-4}}$
   
   $= \frac{f'(x) - f(x)}{e^{x-2}}$

2) $g'(2)$를 구하기 위해 $f'(2)$와 $f(2)$를 알아야 합니다.

3) 주어진 극한 조건을 이용합니다:
   
   $\lim_{x \to 2} \frac{f(x)-3}{x-2} = 5$

   이는 $f'(2) = 5$를 의미하며, $f(2) = 3$임을 알 수 있습니다.

4) 이제 $g'(2)$를 계산할 수 있습니다:

   $g'(2) = \frac{f'(2) - f(2)}{e^{2-2}} = \frac{5 - 3}{e^0} = \frac{2}{1} = 2$

따라서 정답은 **2번: 2**입니다.

## Question 9
For a differentiable function $f(x)$ defined on the set of all real numbers, let the function $g(x)$ be

$g(x) = \frac{f(x)}{e^{x-2}}$

If $\lim_{x \to 2} \frac{f(x)-3}{x-2} = 5$, what is the value of $g'(2)$? **[3 points]**

1. 1
2. 2
3. 3
4. 4
5. 5

### Solution

1) First, let's find the derivative of $g(x)$:

   $g'(x) = \frac{f'(x)e^{x-2} - f(x)e^{x-2}}{(e^{x-2})^2}$
   
   $= \frac{f'(x)e^{x-2} - f(x)e^{x-2}}{e^{2x-4}}$
   
   $= \frac{f'(x) - f(x)}{e^{x-2}}$

2) To find $g'(2)$, we need to know $f'(2)$ and $f(2)$.

3) We can use the given limit condition:
   
   $\lim_{x \to 2} \frac{f(x)-3}{x-2} = 5$

   This implies that $f'(2) = 5$ and $f(2) = 3$.

4) Now we can calculate $g'(2)$:

   $g'(2) = \frac{f'(2) - f(2)}{e^{2-2}} = \frac{5 - 3}{e^0} = \frac{2}{1} = 2$

Therefore, the correct answer is **2: 2**.