

## 문제 25

자연수 $n$에 대하여 다항식 $2x^2 - 3x + 1$을 $x-n$으로 나누었을 때의 나머지를 $a_n$이라 할 때, $\sum_{n=1}^7 (a_n - n^2 + n)$의 값을 구하시오. **[3점]**

### 해설

이 문제를 해결하기 위해 다음 단계를 따릅니다:

1) 다항식을 $x-n$으로 나눈 나머지는 $x=n$일 때의 다항식의 값과 같습니다. 따라서:

   $a_n = 2n^2 - 3n + 1$

2) 주어진 식을 전개합니다:

   $\sum_{n=1}^7 (a_n - n^2 + n)$
   $= \sum_{n=1}^7 ((2n^2 - 3n + 1) - n^2 + n)$
   $= \sum_{n=1}^7 (n^2 - 2n + 1)$

3) 이제 $n=1$부터 $7$까지의 값을 계산하여 합산합니다:

   $n=1: 1^2 - 2(1) + 1 = 0$
   $n=2: 2^2 - 2(2) + 1 = 1$
   $n=3: 3^2 - 2(3) + 1 = 4$
   $n=4: 4^2 - 2(4) + 1 = 9$
   $n=5: 5^2 - 2(5) + 1 = 16$
   $n=6: 6^2 - 2(6) + 1 = 25$
   $n=7: 7^2 - 2(7) + 1 = 36$

4) 이 값들의 합을 구합니다:

   $0 + 1 + 4 + 9 + 16 + 25 + 36 = 91$

따라서, 구하는 값은 91입니다.

## Question 25

For natural numbers $n$, let $a_n$ be the remainder when the polynomial $2x^2 - 3x + 1$ is divided by $x-n$. Find the value of $\sum_{n=1}^7 (a_n - n^2 + n)$. **[3 points]**

### Solution

We can solve this problem using the following steps:

1) The remainder when a polynomial is divided by $x-n$ is equal to the value of the polynomial when $x=n$. Therefore:

   $a_n = 2n^2 - 3n + 1$

2) We expand the given expression:

   $\sum_{n=1}^7 (a_n - n^2 + n)$
   $= \sum_{n=1}^7 ((2n^2 - 3n + 1) - n^2 + n)$
   $= \sum_{n=1}^7 (n^2 - 2n + 1)$

3) Now we calculate the values for $n$ from 1 to 7:

   $n=1: 1^2 - 2(1) + 1 = 0$
   $n=2: 2^2 - 2(2) + 1 = 1$
   $n=3: 3^2 - 2(3) + 1 = 4$
   $n=4: 4^2 - 2(4) + 1 = 9$
   $n=5: 5^2 - 2(5) + 1 = 16$
   $n=6: 6^2 - 2(6) + 1 = 25$
   $n=7: 7^2 - 2(7) + 1 = 36$

4) We sum these values:

   $0 + 1 + 4 + 9 + 16 + 25 + 36 = 91$

Therefore, the required value is 91.