

## 문제 26

함수 $f(x)=(x^2+2)e^{-x}$에 대하여 함수 $g(x)$가 미분가능하고

$g\left(\frac{x+8}{10}\right)=f^{-1}(x)$, $g(1)=0$

을 만족시킬 때, $|g'(1)|$의 값을 구하시오. **[4점]**

### 해설

이 문제를 해결하기 위해 다음 단계를 따릅니다:

1) $f^{-1}(x)$와 $g(x)$ 사이의 관계를 이용합니다.
2) 합성함수의 미분법을 적용합니다.
3) $f'(x)$를 계산합니다.
4) 주어진 조건을 이용하여 필요한 값을 구합니다.

1. $g\left(\frac{x+8}{10}\right)=f^{-1}(x)$ 이므로, $x=f(y)$라 하면 $g\left(\frac{f(y)+8}{10}\right)=y$ 입니다.

2. 양변을 $y$에 대해 미분하면:

   $g'\left(\frac{f(y)+8}{10}\right) \cdot \frac{f'(y)}{10} = 1$

3. $f(x)=(x^2+2)e^{-x}$를 미분하면:
   
   $f'(x) = (2x-x^2-2)e^{-x}$

4. $g(1)=0$이므로, $f(0)=2$입니다. 
   
   위 식에 $y=0$을 대입하면:

   $g'\left(\frac{2+8}{10}\right) \cdot \frac{f'(0)}{10} = 1$
   
   $g'(1) \cdot \frac{-2}{10} = 1$
   
   $g'(1) = -5$

따라서, $|g'(1)| = 5$입니다.

## Question 26

For the function $f(x)=(x^2+2)e^{-x}$, if the function $g(x)$ is differentiable and satisfies

$g\left(\frac{x+8}{10}\right)=f^{-1}(x)$, $g(1)=0$

find the value of $|g'(1)|$. **[4 points]**

### Solution

We'll solve this problem using the following steps:

1) Use the relationship between $f^{-1}(x)$ and $g(x)$.
2) Apply the chain rule for differentiation.
3) Calculate $f'(x)$.
4) Use the given conditions to find the required value.

1. Since $g\left(\frac{x+8}{10}\right)=f^{-1}(x)$, if we let $x=f(y)$, then $g\left(\frac{f(y)+8}{10}\right)=y$.

2. Differentiating both sides with respect to $y$:

   $g'\left(\frac{f(y)+8}{10}\right) \cdot \frac{f'(y)}{10} = 1$

3. Differentiating $f(x)=(x^2+2)e^{-x}$:
   
   $f'(x) = (2x-x^2-2)e^{-x}$

4. Since $g(1)=0$, we have $f(0)=2$. 
   
   Substituting $y=0$ into the equation from step 2:

   $g'\left(\frac{2+8}{10}\right) \cdot \frac{f'(0)}{10} = 1$
   
   $g'(1) \cdot \frac{-2}{10} = 1$
   
   $g'(1) = -5$

Therefore, $|g'(1)| = 5$.