## 문제 12
수열 $\{a_n\}$은 $a_1 = 1$이고, 모든 자연수 $n$에 대하여

$
\sum_{k=1}^{n} (a_k - a_{k+1}) = -n^2 + n
$

을 만족시킨다. $a_{11}$의 값은? **[3점]**

1. 88  
2. 91  
3. 94  
4. 97  
5. 100  

### 해설  
주어진 조건에 따라 $a_n$의 값을 구해봅시다.

1. $\sum_{k=1}^{n} (a_k - a_{k+1})$는 맨 처음 항에서 맨 마지막 항만 남게 되는 망각 합 공식에 따라 $a_1 - a_{n+1}$이 됩니다. 따라서, 
   $
   a_1 - a_{n+1} = -n^2 + n
   $
2. $a_1 = 1$이므로, 식을 정리하면 
   $
   1 - a_{n+1} = -n^2 + n
   $
   $
   a_{n+1} = n^2 - n + 1
   $
3. $n = 10$일 때 $a_{11}$의 값을 구하면,
   $
   a_{11} = 10^2 - 10 + 1 = 100 - 10 + 1 = 91
   $

정답은 **2번: 91**입니다.

## Question 12
The sequence $\{a_n\}$ is given by $a_1 = 1$, and for all natural numbers $n$,

$
\sum_{k=1}^{n} (a_k - a_{k+1}) = -n^2 + n
$

is satisfied. What is the value of $a_{11}$? **[3 points]**

1. 88  
2. 91  
3. 94  
4. 97  
5. 100  

### Solution  
Let's determine the value of $a_n$ based on the given condition.

1. The sum $\sum_{k=1}^{n} (a_k - a_{k+1})$ simplifies to $a_1 - a_{n+1}$ due to the telescoping nature of the series. Therefore,
   $
   a_1 - a_{n+1} = -n^2 + n
   $
2. Given $a_1 = 1$, we rearrange the equation:
   $
   1 - a_{n+1} = -n^2 + n
   $
   $
   a_{n+1} = n^2 - n + 1
   $
3. To find $a_{11}$, substitute $n = 10$:
   $
   a_{11} = 10^2 - 10 + 1 = 100 - 10 + 1 = 91
   $

The correct answer is **2: 91**.
