

## 문제 23
함수 $f(x) = \frac{x^2 - 2x - 6}{x - 1}$에 대하여 $f'(0)$의 값을 구하시오. **[3점]**

### 해설  
함수 $f(x) = \frac{x^2 - 2x - 6}{x - 1}$의 도함수 $f'(x)$를 구한 다음, $x = 0$에서의 값을 계산합니다.

1. 먼저, 주어진 함수 $f(x)$를 단순화합니다.
   $
   f(x) = \frac{(x^2 - 2x - 6)}{(x - 1)}
   $
   이 함수는 분모 $x - 1$로 인한 특이점이 있을 수 있습니다. $f(x)$를 $x-1$로 나눌 수 있도록 식을 변형하면:
   $
   x^2 - 2x - 6 = (x - 1)(x + 1) - 5
   $
   따라서,
   $
   f(x) = x + 1 - \frac{5}{x - 1}
   $
   
2. 이제, $f(x)$의 도함수 $f'(x)$를 구합니다. 
   $
   f'(x) = 1 + \frac{5}{(x - 1)^2}
   $
   
3. $f'(0)$의 값을 계산합니다.
   $
   f'(0) = 1 + \frac{5}{(0 - 1)^2} = 1 + \frac{5}{1} = 1 + 5 = 6
   $

정답은 **6**입니다.

## Question 23 
Find the value of $f'(0)$ for the function $f(x) = \frac{x^2 - 2x - 6}{x - 1}$. **[3 points]**

## Solution  
To find $f'(0)$, first determine the derivative $f'(x)$ of the given function $f(x)$.

1. Simplify the given function $f(x)$:
   $
   f(x) = \frac{x^2 - 2x - 6}{x - 1}
   $
   Notice that the expression $x^2 - 2x - 6$ can be factored as $(x - 1)(x + 1) - 5$:
   $
   f(x) = x + 1 - \frac{5}{x - 1}
   $

2. Differentiate $f(x)$ to find $f'(x)$:
   $
   f'(x) = 1 + \frac{5}{(x - 1)^2}
   $

3. Calculate $f'(0)$:
   $
   f'(0) = 1 + \frac{5}{(0 - 1)^2} = 1 + \frac{5}{1} = 1 + 5 = 6
   $

The correct answer is **6**.