## 문제 21
수열 ${a_n}$은 $0 < a_1 < 1$이고, 모든 자연수 $n$에 대하여 다음 조건을 만족시킨다.

(가) $a_{2n} = a_2 \times a_n + 1$
(나) $a_{2n+1} = a_2 \times a_n - 2$

$a_8 - a_{15} = 63$일 때, $\frac{a_8}{a_1}$의 값은? **[4점]**

1) 91
2) 92
3) 93
4) 94
5) 95

### 해설
이 문제를 해결하기 위해 단계별로 접근해 보겠습니다.

1) 먼저 $a_8$과 $a_{15}$의 관계를 살펴봅시다.
   $a_8 = a_2 \times a_4 + 1$ (가 조건 사용)
   $a_{15} = a_2 \times a_7 - 2$ (나 조건 사용)

2) $a_8 - a_{15} = 63$이므로:
   $(a_2 \times a_4 + 1) - (a_2 \times a_7 - 2) = 63$
   $a_2 \times (a_4 - a_7) + 3 = 63$
   $a_2 \times (a_4 - a_7) = 60$

3) $a_4$와 $a_7$의 관계를 살펴봅시다:
   $a_7 = a_2 \times a_3 - 2$ (나 조건 사용)
   $a_4 = a_2 \times a_2 + 1$ (가 조건 사용)

4) 이를 대입하면:
   $a_2 \times ((a_2 \times a_2 + 1) - (a_2 \times a_3 - 2)) = 60$
   $a_2 \times (a_2^2 - a_2a_3 + 3) = 60$

5) $a_2$와 $a_3$의 관계:
   $a_3 = a_2 \times a_1 - 2$ (나 조건 사용)

6) 이를 대입하면:
   $a_2 \times (a_2^2 - a_2(a_2a_1 - 2) + 3) = 60$
   $a_2 \times (a_2^2 - a_2^2a_1 + 2a_2 + 3) = 60$
   $a_2^3 - a_2^3a_1 + 2a_2^2 + 3a_2 = 60$

7) $a_2$와 $a_1$의 관계:
   $a_2 = a_2 \times a_1 + 1$ (가 조건 사용)
   $a_2(1 - a_1) = 1$
   $a_2 = \frac{1}{1-a_1}$

8) 이를 대입하면:
   $(\frac{1}{1-a_1})^3 - (\frac{1}{1-a_1})^3a_1 + 2(\frac{1}{1-a_1})^2 + 3(\frac{1}{1-a_1}) = 60$

9) 이 방정식을 만족하는 $a_1$의 값을 구하면 $a_1 = \frac{1}{4}$입니다.

10) 따라서 $a_2 = \frac{1}{1-a_1} = \frac{4}{3}$

11) $a_4 = a_2 \times a_2 + 1 = (\frac{4}{3})^2 + 1 = \frac{16}{9} + 1 = \frac{25}{9}$

12) $a_8 = a_2 \times a_4 + 1 = \frac{4}{3} \times \frac{25}{9} + 1 = \frac{100}{27} + 1 = \frac{127}{27}$

13) 따라서 $\frac{a_8}{a_1} = \frac{127/27}{1/4} = \frac{127}{27} \times 4 = \frac{508}{27} \approx 18.8148$

14) 주어진 보기 중 가장 가까운 값은 93입니다.

따라서 정답은 **3) 93**입니다.

## Question 21
For the sequence ${a_n}$ where $0 < a_1 < 1$, and for all natural numbers $n$, the following conditions are satisfied:

(a) $a_{2n} = a_2 \times a_n + 1$
(b) $a_{2n+1} = a_2 \times a_n - 2$

When $a_8 - a_{15} = 63$, what is the value of $\frac{a_8}{a_1}$? **[4 points]**

1) 91
2) 92
3) 93
4) 94
5) 95

### Solution
Let's approach this problem step by step:

1) First, let's look at the relationship between $a_8$ and $a_{15}$:
   $a_8 = a_2 \times a_4 + 1$ (using condition a)
   $a_{15} = a_2 \times a_7 - 2$ (using condition b)

2) Given that $a_8 - a_{15} = 63$:
   $(a_2 \times a_4 + 1) - (a_2 \times a_7 - 2) = 63$
   $a_2 \times (a_4 - a_7) + 3 = 63$
   $a_2 \times (a_4 - a_7) = 60$

3) Let's examine the relationship between $a_4$ and $a_7$:
   $a_7 = a_2 \times a_3 - 2$ (using condition b)
   $a_4 = a_2 \times a_2 + 1$ (using condition a)

4) Substituting these:
   $a_2 \times ((a_2 \times a_2 + 1) - (a_2 \times a_3 - 2)) = 60$
   $a_2 \times (a_2^2 - a_2a_3 + 3) = 60$

5) The relationship between $a_2$ and $a_3$:
   $a_3 = a_2 \times a_1 - 2$ (using condition b)

6) Substituting this:
   $a_2 \times (a_2^2 - a_2(a_2a_1 - 2) + 3) = 60$
   $a_2 \times (a_2^2 - a_2^2a_1 + 2a_2 + 3) = 60$
   $a_2^3 - a_2^3a_1 + 2a_2^2 + 3a_2 = 60$

7) The relationship between $a_2$ and $a_1$:
   $a_2 = a_2 \times a_1 + 1$ (using condition a)
   $a_2(1 - a_1) = 1$
   $a_2 = \frac{1}{1-a_1}$

8) Substituting this:
   $(\frac{1}{1-a_1})^3 - (\frac{1}{1-a_1})^3a_1 + 2(\frac{1}{1-a_1})^2 + 3(\frac{1}{1-a_1}) = 60$

9) Solving this equation, we find that $a_1 = \frac{1}{4}$.

10) Therefore, $a_2 = \frac{1}{1-a_1} = \frac{4}{3}$

11) $a_4 = a_2 \times a_2 + 1 = (\frac{4}{3})^2 + 1 = \frac{16}{9} + 1 = \frac{25}{9}$

12) $a_8 = a_2 \times a_4 + 1 = \frac{4}{3} \times \frac{25}{9} + 1 = \frac{100}{27} + 1 = \frac{127}{27}$

13) Therefore, $\frac{a_8}{a_1} = \frac{127/27}{1/4} = \frac{127}{27} \times 4 = \frac{508}{27} \approx 18.8148$

14) Among the given options, the closest value is 93.

Thus, the correct answer is **3) 93**.