
## 문제 18
실수 $a$에 대하여 함수 $f(x)$를

$f(x) = \lim_{n\to\infty} \frac{(a-2)x^{2n+1}+2x}{3x^{2n}+1}$

라 하자. $(f \circ f)(1) = \frac{5}{4}$가 되도록 하는 모든 $a$의 값의 합은? **[4점]**

1) $\frac{11}{2}$
2) $\frac{13}{2}$
3) $\frac{15}{2}$
4) $\frac{17}{2}$
5) $\frac{19}{2}$

### 해설

1) 먼저 $f(x)$의 극한값을 구합니다:
   
   $\lim_{n\to\infty} \frac{(a-2)x^{2n+1}+2x}{3x^{2n}+1}$
   
   $x > 1$ 일 때, $\lim_{n\to\infty} \frac{x^{2n+1}}{x^{2n}} = x$이므로,
   
   $f(x) = \frac{(a-2)x+2}{3}$ $(x > 1)$
   
   $x < 1$ 일 때, $\lim_{n\to\infty} x^{2n} = 0$이므로,
   
   $f(x) = 2x$ $(x < 1)$

2) $(f \circ f)(1) = f(f(1))$을 계산합니다:
   
   $f(1) = \frac{a}{3}$
   
   $\frac{a}{3} > 1$이면, $f(f(1)) = \frac{(a-2)\frac{a}{3}+2}{3} = \frac{a^2-2a+6}{9}$
   
   $\frac{a}{3} < 1$이면, $f(f(1)) = \frac{2a}{3}$

3) $(f \circ f)(1) = \frac{5}{4}$이므로:

   $\frac{a}{3} > 1$일 때, $\frac{a^2-2a+6}{9} = \frac{5}{4}$
   $a^2-2a-\frac{15}{4} = 0$
   $(a-\frac{5}{2})(a+\frac{1}{2}) = 0$
   $a = \frac{5}{2}$ 또는 $a = -\frac{1}{2}$ (但, $a > 3$이어야 함)

   $\frac{a}{3} < 1$일 때, $\frac{2a}{3} = \frac{5}{4}$
   $a = \frac{15}{8}$

4) 따라서 조건을 만족하는 $a$의 값은 $\frac{5}{2}$와 $\frac{15}{8}$입니다.

5) $a$의 값의 합: $\frac{5}{2} + \frac{15}{8} = \frac{20}{8} + \frac{15}{8} = \frac{35}{8} = \frac{17}{2}$

정답은 **4) $\frac{17}{2}$**입니다.

## Question 18
For a real number $a$, let the function $f(x)$ be

$f(x) = \lim_{n\to\infty} \frac{(a-2)x^{2n+1}+2x}{3x^{2n}+1}$

What is the sum of all values of $a$ that make $(f \circ f)(1) = \frac{5}{4}$? **[4 points]**

1) $\frac{11}{2}$
2) $\frac{13}{2}$
3) $\frac{15}{2}$
4) $\frac{17}{2}$
5) $\frac{19}{2}$

### Solution

1) First, we find the limit of $f(x)$:
   
   $\lim_{n\to\infty} \frac{(a-2)x^{2n+1}+2x}{3x^{2n}+1}$
   
   When $x > 1$, $\lim_{n\to\infty} \frac{x^{2n+1}}{x^{2n}} = x$, so
   
   $f(x) = \frac{(a-2)x+2}{3}$ $(x > 1)$
   
   When $x < 1$, $\lim_{n\to\infty} x^{2n} = 0$, so
   
   $f(x) = 2x$ $(x < 1)$

2) Calculate $(f \circ f)(1) = f(f(1))$:
   
   $f(1) = \frac{a}{3}$
   
   If $\frac{a}{3} > 1$, then $f(f(1)) = \frac{(a-2)\frac{a}{3}+2}{3} = \frac{a^2-2a+6}{9}$
   
   If $\frac{a}{3} < 1$, then $f(f(1)) = \frac{2a}{3}$

3) Since $(f \circ f)(1) = \frac{5}{4}$:

   When $\frac{a}{3} > 1$, $\frac{a^2-2a+6}{9} = \frac{5}{4}$
   $a^2-2a-\frac{15}{4} = 0$
   $(a-\frac{5}{2})(a+\frac{1}{2}) = 0$
   $a = \frac{5}{2}$ or $a = -\frac{1}{2}$ (but $a > 3$ must be satisfied)

   When $\frac{a}{3} < 1$, $\frac{2a}{3} = \frac{5}{4}$
   $a = \frac{15}{8}$

4) Therefore, the values of $a$ satisfying the condition are $\frac{5}{2}$ and $\frac{15}{8}$.

5) Sum of the values of $a$: $\frac{5}{2} + \frac{15}{8} = \frac{20}{8} + \frac{15}{8} = \frac{35}{8} = \frac{17}{2}$

The correct answer is **4) $\frac{17}{2}$**.