

## 문제 1

$\left(2^{\sqrt{3}} \times 4\right)^{\sqrt{3}-2}$의 값은? **[2점]**

1. $\frac{1}{4}$
2. $\frac{1}{2}$
3. 1
4. 2
5. 4

### 해설

주어진 식 $\left(2^{\sqrt{3}} \times 4\right)^{\sqrt{3}-2}$의 값을 계산해봅시다.

1. $2^{\sqrt{3}} \times 4$를 간단히 해봅시다:
   $2^{\sqrt{3}} \times 4 = 2^{\sqrt{3}} \times 2^2 = 2^{\sqrt{3}+2}$

2. 이제 전체 식은 다음과 같이 됩니다:
   $\left(2^{\sqrt{3}+2}\right)^{\sqrt{3}-2}$

3. 지수법칙을 적용하면:
   $2^{(\sqrt{3}+2)(\sqrt{3}-2)} = 2^{\sqrt{3}^2-2^2} = 2^{3-4} = 2^{-1} = \frac{1}{2}$

따라서, $\left(2^{\sqrt{3}} \times 4\right)^{\sqrt{3}-2} = \frac{1}{2}$입니다.

정답은 **2번: $\frac{1}{2}$**입니다.

## Question 1

What is the value of $\left(2^{\sqrt{3}} \times 4\right)^{\sqrt{3}-2}$? **[2 points]**

1. $\frac{1}{4}$
2. $\frac{1}{2}$
3. 1
4. 2
5. 4

### Solution

Let's calculate the value of the expression $\left(2^{\sqrt{3}} \times 4\right)^{\sqrt{3}-2}$.

1. First, simplify $2^{\sqrt{3}} \times 4$:
   $2^{\sqrt{3}} \times 4 = 2^{\sqrt{3}} \times 2^2 = 2^{\sqrt{3}+2}$

2. Now the entire expression becomes:
   $\left(2^{\sqrt{3}+2}\right)^{\sqrt{3}-2}$

3. Applying the laws of exponents:
   $2^{(\sqrt{3}+2)(\sqrt{3}-2)} = 2^{\sqrt{3}^2-2^2} = 2^{3-4} = 2^{-1} = \frac{1}{2}$

Therefore, $\left(2^{\sqrt{3}} \times 4\right)^{\sqrt{3}-2} = \frac{1}{2}$.

The correct answer is **2: $\frac{1}{2}$**.