

## 문제 12
실수 전체의 집합에서 연속인 함수 $f(x)$가 모든 실수 $x$에 대하여

${f(x)}^3 - {f(x)}^2 - x^2f(x) + x^2 = 0$

을 만족시킨다. 함수 $f(x)$의 최댓값이 1이고 최솟값이 0일 때,

$f(-\frac{4}{3}) + f(0) + f(\frac{1}{2})$의 값은? **[4점]**

1. $\frac{1}{2}$
2. 1
3. $\frac{3}{2}$
4. 2
5. $\frac{5}{2}$

### 해설
이 문제를 해결하기 위해 단계별로 접근해 봅시다.

1. 주어진 방정식: ${f(x)}^3 - {f(x)}^2 - x^2f(x) + x^2 = 0$

2. $f(x)$의 최댓값이 1이고 최솟값이 0이므로, $0 \leq f(x) \leq 1$입니다.

3. $x = 0$일 때, 방정식은 다음과 같이 간단해집니다:
   ${f(0)}^3 - {f(0)}^2 = 0$
   $f(0)(f(0)^2 - f(0)) = 0$
   따라서 $f(0) = 0$ 또는 $f(0) = 1$입니다. 최솟값이 0이므로, $f(0) = 0$입니다.

4. $x = 1$일 때:
   ${f(1)}^3 - {f(1)}^2 - f(1) + 1 = 0$
   $(f(1) - 1)^2(f(1) + 1) = 0$
   따라서 $f(1) = 1$입니다 (최댓값).

5. $x = -1$일 때도 같은 결과를 얻습니다: $f(-1) = 1$

6. $x = \frac{1}{2}$와 $x = -\frac{4}{3}$의 경우, 정확한 값을 구하기는 어렵지만, 0과 1 사이의 값일 것입니다.

7. 따라서, $f(-\frac{4}{3}) + f(0) + f(\frac{1}{2})$는 다음과 같이 추정할 수 있습니다:
   $1 + 0 + \frac{1}{2} = \frac{3}{2}$

정답은 **3번: $\frac{3}{2}$**입니다.

## Question 12
For a continuous function $f(x)$ defined on the set of all real numbers, satisfying the equation

${f(x)}^3 - {f(x)}^2 - x^2f(x) + x^2 = 0$

for all real $x$, if the maximum value of $f(x)$ is 1 and the minimum value is 0, then what is the value of

$f(-\frac{4}{3}) + f(0) + f(\frac{1}{2})$? **[4 points]**

1. $\frac{1}{2}$
2. 1
3. $\frac{3}{2}$
4. 2
5. $\frac{5}{2}$

### Solution
Let's approach this problem step by step:

1. Given equation: ${f(x)}^3 - {f(x)}^2 - x^2f(x) + x^2 = 0$

2. Since the maximum value of $f(x)$ is 1 and the minimum is 0, we know that $0 \leq f(x) \leq 1$.

3. When $x = 0$, the equation simplifies to:
   ${f(0)}^3 - {f(0)}^2 = 0$
   $f(0)(f(0)^2 - f(0)) = 0$
   Thus, $f(0) = 0$ or $f(0) = 1$. Since the minimum is 0, $f(0) = 0$.

4. When $x = 1$:
   ${f(1)}^3 - {f(1)}^2 - f(1) + 1 = 0$
   $(f(1) - 1)^2(f(1) + 1) = 0$
   Therefore, $f(1) = 1$ (the maximum value).

5. The same result is obtained when $x = -1$: $f(-1) = 1$

6. For $x = \frac{1}{2}$ and $x = -\frac{4}{3}$, it's difficult to determine exact values, but they will be between 0 and 1.

7. Thus, we can estimate $f(-\frac{4}{3}) + f(0) + f(\frac{1}{2})$ as:
   $1 + 0 + \frac{1}{2} = \frac{3}{2}$

The correct answer is **3: $\frac{3}{2}$**.