

## 문제 18
두 수열 ${a_n}$, ${b_n}$에 대하여

$\sum_{k=1}^{10} a_k = \sum_{k=1}^{10} (2b_k - 1)$, $\sum_{k=1}^{10} (3a_k + b_k) = 33$

일 때, $\sum_{k=1}^{10} b_k$의 값을 구하시오. **[3점]**

### 해설
주어진 식을 이용하여 단계별로 풀어봅시다.

1. 첫 번째 식: $\sum_{k=1}^{10} a_k = \sum_{k=1}^{10} (2b_k - 1)$
   $\sum_{k=1}^{10} a_k = 2\sum_{k=1}^{10} b_k - 10$

2. 두 번째 식: $\sum_{k=1}^{10} (3a_k + b_k) = 33$
   $3\sum_{k=1}^{10} a_k + \sum_{k=1}^{10} b_k = 33$

3. 첫 번째 식을 이용하여 $\sum_{k=1}^{10} a_k$를 두 번째 식에 대입:
   $3(2\sum_{k=1}^{10} b_k - 10) + \sum_{k=1}^{10} b_k = 33$

4. 식을 전개:
   $6\sum_{k=1}^{10} b_k - 30 + \sum_{k=1}^{10} b_k = 33$
   $7\sum_{k=1}^{10} b_k - 30 = 33$
   $7\sum_{k=1}^{10} b_k = 63$

5. 최종 계산:
   $\sum_{k=1}^{10} b_k = 63 \div 7 = 9$

따라서, $\sum_{k=1}^{10} b_k$의 값은 **9**입니다.

## Question 18
For two sequences ${a_n}$ and ${b_n}$,

$\sum_{k=1}^{10} a_k = \sum_{k=1}^{10} (2b_k - 1)$, $\sum_{k=1}^{10} (3a_k + b_k) = 33$

Find the value of $\sum_{k=1}^{10} b_k$. **[3 points]**

### Solution
Let's solve this step by step using the given equations.

1. From the first equation: $\sum_{k=1}^{10} a_k = \sum_{k=1}^{10} (2b_k - 1)$
   $\sum_{k=1}^{10} a_k = 2\sum_{k=1}^{10} b_k - 10$

2. From the second equation: $\sum_{k=1}^{10} (3a_k + b_k) = 33$
   $3\sum_{k=1}^{10} a_k + \sum_{k=1}^{10} b_k = 33$

3. Substitute $\sum_{k=1}^{10} a_k$ from the first equation into the second:
   $3(2\sum_{k=1}^{10} b_k - 10) + \sum_{k=1}^{10} b_k = 33$

4. Expand the equation:
   $6\sum_{k=1}^{10} b_k - 30 + \sum_{k=1}^{10} b_k = 33$
   $7\sum_{k=1}^{10} b_k - 30 = 33$
   $7\sum_{k=1}^{10} b_k = 63$

5. Final calculation:
   $\sum_{k=1}^{10} b_k = 63 \div 7 = 9$

Therefore, the value of $\sum_{k=1}^{10} b_k$ is **9**.