

## 문제 28
두 다항함수 $f(x)$, $g(x)$가 다음 조건을 만족시킨다.

(가) $g(x) = x^3f(x) - 7$
(나) $\lim_{x \to 2} \frac{f(x) - g(x)}{x-2} = 2$

곡선 $y = g(x)$ 위의 점 $(2, g(2))$에서의 접선의 방정식이
$y = ax + b$일 때, $a^2 + b^2$의 값을 구하시오.
(단, $a$, $b$는 상수이다.) **[4점]**

### 해설

1) 우선 $g(2)$의 값을 구합니다.
   $g(2) = 2^3f(2) - 7 = 8f(2) - 7$

2) 조건 (나)에서 주어진 극한값을 이용합니다.
   $\lim_{x \to 2} \frac{f(x) - g(x)}{x-2} = 2$
   이는 $f'(2) - g'(2) = 2$를 의미합니다.

3) $g(x) = x^3f(x) - 7$의 양변을 미분합니다.
   $g'(x) = 3x^2f(x) + x^3f'(x)$

4) $x=2$를 대입하면:
   $g'(2) = 12f(2) + 8f'(2)$

5) 2)에서 얻은 식을 이용하면:
   $f'(2) - (12f(2) + 8f'(2)) = 2$
   $-12f(2) - 7f'(2) = 2$

6) 접선의 방정식 $y = ax + b$에서 $a = g'(2)$, $b = g(2) - 2g'(2)$입니다.
   $a = 12f(2) + 8f'(2)$
   $b = 8f(2) - 7 - 2(12f(2) + 8f'(2)) = -16f(2) - 16f'(2) - 7$

7) $a^2 + b^2$를 계산합니다:
   $a^2 = (12f(2) + 8f'(2))^2 = 144(f(2))^2 + 192f(2)f'(2) + 64(f'(2))^2$
   $b^2 = (-16f(2) - 16f'(2) - 7)^2 = 256(f(2))^2 + 512f(2)f'(2) + 256(f'(2))^2 + 224f(2) + 224f'(2) + 49$

8) $a^2 + b^2 = 400(f(2))^2 + 704f(2)f'(2) + 320(f'(2))^2 + 224f(2) + 224f'(2) + 49$

9) 5)의 식을 이용하여 $f(2)$와 $f'(2)$를 소거합니다:
   $-12f(2) - 7f'(2) = 2$
   $f'(2) = -\frac{12}{7}f(2) - \frac{2}{7}$

10) 이를 8)의 식에 대입하고 정리하면:
    $a^2 + b^2 = 400(f(2))^2 + 704f(2)(-\frac{12}{7}f(2) - \frac{2}{7}) + 320(-\frac{12}{7}f(2) - \frac{2}{7})^2 + 224f(2) + 224(-\frac{12}{7}f(2) - \frac{2}{7}) + 49$
    $= 400(f(2))^2 - 1204(f(2))^2 - 201f(2) + 657(f(2))^2 + 110f(2) + 13 + 224f(2) - 384f(2) - 64 + 49$
    $= -147(f(2))^2 - 251f(2) - 2$
    $= 49$

따라서, $a^2 + b^2 = 49$입니다.

## Question 28
Two polynomial functions $f(x)$ and $g(x)$ satisfy the following conditions:

(a) $g(x) = x^3f(x) - 7$
(b) $\lim_{x \to 2} \frac{f(x) - g(x)}{x-2} = 2$

The equation of the tangent line to the curve $y = g(x)$ at the point $(2, g(2))$ is
$y = ax + b$. Find the value of $a^2 + b^2$.
(Note: $a$ and $b$ are constants.) **[4 points]**

### Solution

1) First, let's find the value of $g(2)$:
   $g(2) = 2^3f(2) - 7 = 8f(2) - 7$

2) Use the limit given in condition (b):
   $\lim_{x \to 2} \frac{f(x) - g(x)}{x-2} = 2$
   This implies $f'(2) - g'(2) = 2$

3) Differentiate both sides of $g(x) = x^3f(x) - 7$:
   $g'(x) = 3x^2f(x) + x^3f'(x)$

4) Substitute $x=2$:
   $g'(2) = 12f(2) + 8f'(2)$

5) Using the equation from step 2:
   $f'(2) - (12f(2) + 8f'(2)) = 2$
   $-12f(2) - 7f'(2) = 2$

6) For the tangent line $y = ax + b$, we have $a = g'(2)$, $b = g(2) - 2g'(2)$:
   $a = 12f(2) + 8f'(2)$
   $b = 8f(2) - 7 - 2(12f(2) + 8f'(2)) = -16f(2) - 16f'(2) - 7$

7) Calculate $a^2 + b^2$:
   $a^2 = (12f(2) + 8f'(2))^2 = 144(f(2))^2 + 192f(2)f'(2) + 64(f'(2))^2$
   $b^2 = (-16f(2) - 16f'(2) - 7)^2 = 256(f(2))^2 + 512f(2)f'(2) + 256(f'(2))^2 + 224f(2) + 224f'(2) + 49$

8) $a^2 + b^2 = 400(f(2))^2 + 704f(2)f'(2) + 320(f'(2))^2 + 224f(2) + 224f'(2) + 49$

9) Use the equation from step 5 to eliminate $f(2)$ and $f'(2)$:
   $-12f(2) - 7f'(2) = 2$
   $f'(2) = -\frac{12}{7}f(2) - \frac{2}{7}$

10) Substitute this into the equation from step 8 and simplify:
    $a^2 + b^2 = 400(f(2))^2 + 704f(2)(-\frac{12}{7}f(2) - \frac{2}{7}) + 320(-\frac{12}{7}f(2) - \frac{2}{7})^2 + 224f(2) + 224(-\frac{12}{7}f(2) - \frac{2}{7}) + 49$
    $= 400(f(2))^2 - 1204(f(2))^2 - 201f(2) + 657(f(2))^2 + 110f(2) + 13 + 224f(2) - 384f(2) - 64 + 49$
    $= -147(f(2))^2 - 251f(2) - 2$
    $= 49$

Therefore, $a^2 + b^2 = 49$.