

## 문제 18
최고차항의 계수가 1이고 $f(1)=0$인 삼차함수 $f(x)$가

$\lim_{x \to 2} \frac{f(x)}{(x-2)\{f'(x)\}^2} = \frac{1}{4}$

을 만족시킬 때, $f(3)$의 값은? **[4점]**

1) 4
2) 6
3) 8
4) 10
5) 12

### 해설
이 문제를 해결하기 위해 단계별로 접근해 보겠습니다.

1) $f(x)$는 최고차항의 계수가 1인 삼차함수이므로, 일반형은 다음과 같습니다:
   $f(x) = x^3 + ax^2 + bx + c$

2) $f(1) = 0$이므로:
   $1 + a + b + c = 0$ ... (식 1)

3) 주어진 극한 조건을 이용합니다:
   $\lim_{x \to 2} \frac{f(x)}{(x-2)\{f'(x)\}^2} = \frac{1}{4}$

   이는 $x=2$에서 함수가 0이 됨을 의미합니다. 즉, $f(2) = 0$:
   $8 + 4a + 2b + c = 0$ ... (식 2)

4) $f'(x) = 3x^2 + 2ax + b$이므로, $f'(2) = 12 + 4a + b$

5) 극한 조건을 만족하려면:
   $\frac{f'''(2)}{6\{f'(2)\}^2} = \frac{1}{4}$

   $f'''(x) = 6$이므로:
   $\frac{6}{6(12 + 4a + b)^2} = \frac{1}{4}$

   $(12 + 4a + b)^2 = 4$
   $12 + 4a + b = 2$ ... (식 3)

6) 식 1, 2, 3을 연립하여 풀면:
   $a = -3, b = 3, c = -1$

7) 따라서 $f(x) = x^3 - 3x^2 + 3x - 1$

8) $f(3)$을 계산하면:
   $f(3) = 27 - 27 + 9 - 1 = 8$

따라서 정답은 **3) 8**입니다.

## Question 18
For a cubic function $f(x)$ with the highest degree coefficient of 1 and $f(1)=0$, if it satisfies

$\lim_{x \to 2} \frac{f(x)}{(x-2)\{f'(x)\}^2} = \frac{1}{4}$

what is the value of $f(3)$? **[4 points]**

1) 4
2) 6
3) 8
4) 10
5) 12

### Solution
Let's approach this problem step by step:

1) Since $f(x)$ is a cubic function with the highest degree coefficient of 1, its general form is:
   $f(x) = x^3 + ax^2 + bx + c$

2) Given $f(1) = 0$:
   $1 + a + b + c = 0$ ... (Equation 1)

3) Using the given limit condition:
   $\lim_{x \to 2} \frac{f(x)}{(x-2)\{f'(x)\}^2} = \frac{1}{4}$

   This implies that the function becomes 0 at $x=2$. So, $f(2) = 0$:
   $8 + 4a + 2b + c = 0$ ... (Equation 2)

4) $f'(x) = 3x^2 + 2ax + b$, so $f'(2) = 12 + 4a + b$

5) To satisfy the limit condition:
   $\frac{f'''(2)}{6\{f'(2)\}^2} = \frac{1}{4}$

   Since $f'''(x) = 6$:
   $\frac{6}{6(12 + 4a + b)^2} = \frac{1}{4}$

   $(12 + 4a + b)^2 = 4$
   $12 + 4a + b = 2$ ... (Equation 3)

6) Solving Equations 1, 2, and 3 simultaneously:
   $a = -3, b = 3, c = -1$

7) Therefore, $f(x) = x^3 - 3x^2 + 3x - 1$

8) Calculating $f(3)$:
   $f(3) = 27 - 27 + 9 - 1 = 8$

Thus, the correct answer is **3) 8**.