
## 문제 28
두 상수 $a$, $b(a<b)$에 대하여 함수 $f(x)$를

$f(x)=(x-a)(x-b)^2$

이라 하자. 함수 $g(x)=x^3+x+1$의 역함수 $g^{-1}(x)$에 대하여 합성함수 $h(x)=(f \circ g^{-1})(x)$가 다음 조건을 만족시킬 때, $f(8)$의 값을 구하시오. [4점]

(가) 함수 $(x-1)|h(x)|$가 실수 전체의 집합에서 미분가능하다.
(나) $h'(3)=2$

### 해설

1) 조건 (가)에서 $|h(x)|$가 실수 전체의 집합에서 미분가능하려면, $h(1)=0$이어야 합니다.

2) $h(x) = (f \circ g^{-1})(x) = f(g^{-1}(x))$이므로, $h(1) = f(g^{-1}(1)) = 0$입니다.

3) $g(0) = 0^3 + 0 + 1 = 1$이므로, $g^{-1}(1) = 0$입니다.

4) 따라서, $f(0) = 0$이어야 합니다. 이는 $a = 0$ 또는 $b = 0$일 때 성립합니다.

5) $a < b$이므로, $a = 0$이고 $b > 0$입니다.

6) 이제 $f(x) = x(x-b)^2$입니다.

7) 조건 (나)에서 $h'(3) = 2$입니다. 이를 이용해 $b$의 값을 구할 수 있습니다.

8) $h'(x) = f'(g^{-1}(x)) \cdot (g^{-1})'(x)$

9) $(g^{-1})'(x) = \frac{1}{g'(g^{-1}(x))} = \frac{1}{3(g^{-1}(x))^2 + 1}$

10) $f'(x) = (x-b)^2 + 2x(x-b) = 3x^2 - 4bx + b^2$

11) $h'(3) = f'(g^{-1}(3)) \cdot (g^{-1})'(3) = 2$

12) $g(2) = 2^3 + 2 + 1 = 11$이므로, $g^{-1}(3) = 2$입니다.

13) $(3(2)^2 - 4b(2) + b^2) \cdot \frac{1}{3(2)^2 + 1} = 2$

14) $(12 - 8b + b^2) \cdot \frac{1}{13} = 2$

15) $12 - 8b + b^2 = 26$
    $b^2 - 8b + 14 = 0$
    $(b-2)(b-6) = 0$

16) $b > 0$이므로, $b = 6$입니다.

17) 따라서, $f(x) = x(x-6)^2$입니다.

18) $f(8) = 8(8-6)^2 = 8 \cdot 2^2 = 32$

따라서, $f(8) = 32$입니다.

## Question 28
For two constants $a$, $b(a<b)$, let the function $f(x)$ be

$f(x)=(x-a)(x-b)^2$

Let $g(x)=x^3+x+1$ and $g^{-1}(x)$ be its inverse function. If the composite function $h(x)=(f \circ g^{-1})(x)$ satisfies the following conditions, find the value of $f(8)$. [4 points]

(a) The function $(x-1)|h(x)|$ is differentiable on the set of all real numbers.
(b) $h'(3)=2$

### Solution

1) From condition (a), for $|h(x)|$ to be differentiable on the set of all real numbers, we must have $h(1)=0$.

2) Since $h(x) = (f \circ g^{-1})(x) = f(g^{-1}(x))$, we have $h(1) = f(g^{-1}(1)) = 0$.

3) As $g(0) = 0^3 + 0 + 1 = 1$, we have $g^{-1}(1) = 0$.

4) Therefore, we must have $f(0) = 0$. This occurs when $a = 0$ or $b = 0$.

5) Since $a < b$, we have $a = 0$ and $b > 0$.

6) Now, $f(x) = x(x-b)^2$.

7) From condition (b), $h'(3) = 2$. We can use this to find the value of $b$.

8) $h'(x) = f'(g^{-1}(x)) \cdot (g^{-1})'(x)$

9) $(g^{-1})'(x) = \frac{1}{g'(g^{-1}(x))} = \frac{1}{3(g^{-1}(x))^2 + 1}$

10) $f'(x) = (x-b)^2 + 2x(x-b) = 3x^2 - 4bx + b^2$

11) $h'(3) = f'(g^{-1}(3)) \cdot (g^{-1})'(3) = 2$

12) As $g(2) = 2^3 + 2 + 1 = 11$, we have $g^{-1}(3) = 2$.

13) $(3(2)^2 - 4b(2) + b^2) \cdot \frac{1}{3(2)^2 + 1} = 2$

14) $(12 - 8b + b^2) \cdot \frac{1}{13} = 2$

15) $12 - 8b + b^2 = 26$
    $b^2 - 8b + 14 = 0$
    $(b-2)(b-6) = 0$

16) Since $b > 0$, we have $b = 6$.

17) Therefore, $f(x) = x(x-6)^2$.

18) $f(8) = 8(8-6)^2 = 8 \cdot 2^2 = 32$

Thus, $f(8) = 32$.