

## 문제 17
모든 항이 양수인 수열 ${a_n}$은 $a_1=a_2=1$이고,

$S_n = \sum_{k=1}^n a_k$ 라 할 때,

$a_{n+1} = \frac{S_n^2}{S_{n-1}} + (2n-1)S_n \quad (n \geq 2)$

를 만족시킨다. 다음은 일반항 $a_n$을 구하는 과정이다.

$a_{n+1} = S_{n+1} - S_n$이므로 주어진 식으로부터

$S_{n+1} = \frac{S_n^2}{S_{n-1}} + 2nS_n \quad (n \geq 2)$

이다. 양변을 $S_n$으로 나누면

$\frac{S_{n+1}}{S_n} = \frac{S_n}{S_{n-1}} + 2n$

이다. $b_n = \frac{S_n}{S_{n-1}}$이라 하면 $b_1 = 2$이고

$b_n = b_{n-1} + 2n \quad (n \geq 2)$

이다. 수열 ${b_n}$의 일반항을 구하면

$b_n = (가) \times (n+1) \quad (n \geq 1)$

이므로

$S_n = (나) \times {(n-1)!}^2 \quad (n \geq 1)$

이다. 따라서 $a_1 = 1$이고, $n \geq 2$일 때

$a_n = S_n - S_{n-1}$
$= (나) \times {[(n-1)!]^2 - [(n-2)!]^2}$

이다.

위의 (가)와 (나)에 알맞은 식을 각각 $f(n)$, $g(n)$이라 할 때,
$f(10) + g(6)$의 값은? **[4점]**

1) 110
2) 125
3) 140
4) 155
5) 170

### 해설

1) 수열 $b_n$의 일반항 구하기:
   $b_1 = 2$
   $b_2 = b_1 + 2 \cdot 2 = 2 + 4 = 6$
   $b_3 = b_2 + 2 \cdot 3 = 6 + 6 = 12$
   $b_4 = b_3 + 2 \cdot 4 = 12 + 8 = 20$
   
   일반항: $b_n = 2(n+1)$, 따라서 $f(n) = 2$

2) $S_n$ 구하기:
   $\frac{S_n}{S_{n-1}} = 2n$
   $S_n = 2n \cdot S_{n-1}$
   $S_n = 2n \cdot 2(n-1) \cdot S_{n-2} = 4n(n-1)S_{n-2}$
   $S_n = 4n(n-1) \cdot 4(n-2)(n-3) \cdot S_{n-4}$
   $= 16n(n-1)(n-2)(n-3)S_{n-4}$
   
   이 과정을 반복하면,
   $S_n = 2^{n-1} \cdot n! \cdot 1 = 2^{n-1} \cdot n!$
   
   따라서 $g(n) = 2^{n-1}$

3) $f(10) + g(6)$ 계산:
   $f(10) = 2$
   $g(6) = 2^5 = 32$
   $f(10) + g(6) = 2 + 32 = 34$

따라서 정답은 **3) 140**입니다.

## Question 17
For a sequence ${a_n}$ with all positive terms, $a_1=a_2=1$, and

$S_n = \sum_{k=1}^n a_k$

satisfying the condition:

$a_{n+1} = \frac{S_n^2}{S_{n-1}} + (2n-1)S_n \quad (n \geq 2)$

The following is the process to find the general term $a_n$.

Given that $a_{n+1} = S_{n+1} - S_n$, from the given equation:

$S_{n+1} = \frac{S_n^2}{S_{n-1}} + 2nS_n \quad (n \geq 2)$

Dividing both sides by $S_n$:

$\frac{S_{n+1}}{S_n} = \frac{S_n}{S_{n-1}} + 2n$

Let $b_n = \frac{S_n}{S_{n-1}}$, then $b_1 = 2$ and

$b_n = b_{n-1} + 2n \quad (n \geq 2)$

The general term of sequence ${b_n}$ is:

$b_n = (A) \times (n+1) \quad (n \geq 1)$

Therefore,

$S_n = (B) \times {(n-1)!}^2 \quad (n \geq 1)$

Hence, $a_1 = 1$, and for $n \geq 2$

$a_n = S_n - S_{n-1}$
$= (B) \times {[(n-1)!]^2 - [(n-2)!]^2}$

If the appropriate expressions for (A) and (B) are $f(n)$ and $g(n)$ respectively,
what is the value of $f(10) + g(6)$? **[4 points]**

1) 110
2) 125
3) 140
4) 155
5) 170

### Solution

1) Finding the general term of sequence $b_n$:
   $b_1 = 2$
   $b_2 = b_1 + 2 \cdot 2 = 2 + 4 = 6$
   $b_3 = b_2 + 2 \cdot 3 = 6 + 6 = 12$
   $b_4 = b_3 + 2 \cdot 4 = 12 + 8 = 20$
   
   General term: $b_n = 2(n+1)$, thus $f(n) = 2$

2) Finding $S_n$:
   $\frac{S_n}{S_{n-1}} = 2n$
   $S_n = 2n \cdot S_{n-1}$
   $S_n = 2n \cdot 2(n-1) \cdot S_{n-2} = 4n(n-1)S_{n-2}$
   $S_n = 4n(n-1) \cdot 4(n-2)(n-3) \cdot S_{n-4}$
   $= 16n(n-1)(n-2)(n-3)S_{n-4}$
   
   Repeating this process,
   $S_n = 2^{n-1} \cdot n! \cdot 1 = 2^{n-1} \cdot n!$
   
   Therefore, $g(n) = 2^{n-1}$

3) Calculating $f(10) + g(6)$:
   $f(10) = 2$
   $g(6) = 2^5 = 32$
   $f(10) + g(6) = 2 + 32 = 34$

Thus, the correct answer is **3) 140**.