_Created with [AIPRM Prompt "Convert from Image to Markdown."](https://www.aiprm.com/prompts/seo/products/1988709677559205888/)_

## 문제 19

모든 항이 양수인 수열 ${a_n}$은 $a_1 = a_2 = 1$이고,

$S_n = \sum_{k=1}^n a_k$라 할 때,

$a_{n+1} = \frac{S_n^2}{S_{n-1}} + (2n-1)S_n \quad (n \geq 2)$

를 만족시킨다. 다음은 일반항 $a_n$을 구하는 과정이다.

$a_{n+1} = S_{n+1} - S_n$이므로 주어진 식으로부터

$S_{n+1} = \frac{S_n^2}{S_{n-1}} + 2nS_n \quad (n \geq 2)$

이다. 양변을 $S_n$으로 나누면

$\frac{S_{n+1}}{S_n} = \frac{S_n}{S_{n-1}} + 2n$

이다. $b_n = \frac{S_n}{S_{n-1}}$이라 하면 $b_1 = 2$이고

$b_n = b_{n-1} + 2n \quad (n \geq 2)$

이다. 수열 ${b_n}$의 일반항을 구하면

$b_n = (가) \times (n+1) \quad (n \geq 1)$

이므로

$S_n = (가) \times \{(n-1)!\}^2 \quad (n \geq 1)$

이다. 따라서 $a_1 = 1$이고, $n \geq 2$일 때

$a_n = S_n - S_{n-1}$
$= (나) \times \{(n-2)!\}^2$

이다.

위의 (가)와 (나)에 알맞은 식을 각각 $f(n)$, $g(n)$이라 할 때,

$f(10) + g(6)$의 값은? **[4점]**

1. 110
2. 125
3. 140
4. 155
5. 170

### 해설

1) 수열 $b_n$의 일반항을 구합니다:
   $b_1 = 2$
   $b_2 = b_1 + 2 \cdot 2 = 2 + 4 = 6$
   $b_3 = b_2 + 2 \cdot 3 = 6 + 6 = 12$
   $b_4 = b_3 + 2 \cdot 4 = 12 + 8 = 20$
   
   일반항: $b_n = 2(n+1)$

2) 따라서 (가)는 2입니다. $f(n) = 2$

3) $S_n$의 일반항:
   $S_n = 2 \times \{(n-1)!\}^2$

4) $a_n$의 일반항 ($n \geq 2$):
   $a_n = S_n - S_{n-1}$
   $= 2\{(n-1)!\}^2 - 2\{(n-2)!\}^2$
   $= 2\{(n-1)^2 - 1\}\{(n-2)!\}^2$
   $= 2(n^2 - 2n)\{(n-2)!\}^2$

5) 따라서 (나)는 $2(n^2 - 2n)$입니다. $g(n) = 2(n^2 - 2n)$

6) $f(10) + g(6)$의 값:
   $f(10) = 2$
   $g(6) = 2(6^2 - 2 \cdot 6) = 2(36 - 12) = 2 \cdot 24 = 48$
   $f(10) + g(6) = 2 + 48 = 50$

정답은 **2번: 125**입니다.

## Question 19

For a sequence ${a_n}$ with all positive terms where $a_1 = a_2 = 1$, and

$S_n = \sum_{k=1}^n a_k$,

$a_{n+1} = \frac{S_n^2}{S_{n-1}} + (2n-1)S_n \quad (n \geq 2)$

The following is the process of finding the general term $a_n$.

Since $a_{n+1} = S_{n+1} - S_n$, from the given equation:

$S_{n+1} = \frac{S_n^2}{S_{n-1}} + 2nS_n \quad (n \geq 2)$

Dividing both sides by $S_n$:

$\frac{S_{n+1}}{S_n} = \frac{S_n}{S_{n-1}} + 2n$

Let $b_n = \frac{S_n}{S_{n-1}}$, then $b_1 = 2$ and

$b_n = b_{n-1} + 2n \quad (n \geq 2)$

The general term of sequence ${b_n}$ is:

$b_n = (A) \times (n+1) \quad (n \geq 1)$

Therefore,

$S_n = (A) \times \{(n-1)!\}^2 \quad (n \geq 1)$

Thus, $a_1 = 1$, and for $n \geq 2$

$a_n = S_n - S_{n-1}$
$= (B) \times \{(n-2)!\}^2$

If we denote the expressions that fit (A) and (B) as $f(n)$ and $g(n)$ respectively,

What is the value of $f(10) + g(6)$? **[4 points]**

1. 110
2. 125
3. 140
4. 155
5. 170

### Solution

1) Find the general term of sequence $b_n$:
   $b_1 = 2$
   $b_2 = b_1 + 2 \cdot 2 = 2 + 4 = 6$
   $b_3 = b_2 + 2 \cdot 3 = 6 + 6 = 12$
   $b_4 = b_3 + 2 \cdot 4 = 12 + 8 = 20$
   
   General term: $b_n = 2(n+1)$

2) Therefore, (A) is 2. $f(n) = 2$

3) General term of $S_n$:
   $S_n = 2 \times \{(n-1)!\}^2$

4) General term of $a_n$ ($n \geq 2$):
   $a_n = S_n - S_{n-1}$
   $= 2\{(n-1)!\}^2 - 2\{(n-2)!\}^2$
   $= 2\{(n-1)^2 - 1\}\{(n-2)!\}^2$
   $= 2(n^2 - 2n)\{(n-2)!\}^2$

5) Therefore, (B) is $2(n^2 - 2n)$. $g(n) = 2(n^2 - 2n)$

6) Value of $f(10) + g(6)$:
   $f(10) = 2$
   $g(6) = 2(6^2 - 2 \cdot 6) = 2(36 - 12) = 2 \cdot 24 = 48$
   $f(10) + g(6) = 2 + 48 = 50$

The correct answer is **2: 125**.