

## 문제 17
자연수 $n$의 양의 약수의 개수를 $f(n)$이라 하고, 36의 모든 양의 약수를 $a_1, a_2, a_3, \cdots, a_9$라 하자.

$\sum_{k=1}^9 \left\{(-1)^{f(a_k)} \times \log a_k\right\}$의 값은? **[4점]**

1. $\log 2 + \log 3$
2. $2\log 2 + \log 3$
3. $\log 2 + 2\log 3$
4. $2\log 2 + 2\log 3$
5. $3\log 2 + 2\log 3$

### 해설
이 문제를 해결하기 위해 단계별로 접근해 보겠습니다.

1. 먼저 36의 모든 양의 약수를 나열합니다:
   $a_1 = 1, a_2 = 2, a_3 = 3, a_4 = 4, a_5 = 6, a_6 = 9, a_7 = 12, a_8 = 18, a_9 = 36$

2. 각 약수에 대해 $f(a_k)$를 구합니다:
   - $f(1) = 1$
   - $f(2) = 2$
   - $f(3) = 2$
   - $f(4) = 3$
   - $f(6) = 4$
   - $f(9) = 3$
   - $f(12) = 6$
   - $f(18) = 6$
   - $f(36) = 9$

3. 이제 주어진 식을 계산합니다:
   $\sum_{k=1}^9 \left\{(-1)^{f(a_k)} \times \log a_k\right\}$
   $= (-1)^1 \log 1 + (-1)^2 \log 2 + (-1)^2 \log 3 + (-1)^3 \log 4 + (-1)^4 \log 6$
   $+ (-1)^3 \log 9 + (-1)^6 \log 12 + (-1)^6 \log 18 + (-1)^9 \log 36$

4. $\log 1 = 0$이므로 첫 항은 무시할 수 있습니다. 또한 짝수 지수의 $(-1)$은 1이 되고, 홀수 지수의 $(-1)$은 -1이 됩니다:
   $= \log 2 + \log 3 - \log 4 + \log 6 - \log 9 + \log 12 + \log 18 - \log 36$

5. 로그 법칙을 이용하여 정리합니다:
   $= \log 2 + \log 3 - \log 2^2 + \log (2 \times 3) - \log 3^2 + \log (2^2 \times 3) + \log (2 \times 3^2) - \log (2^2 \times 3^2)$
   $= \log 2 + \log 3 - 2\log 2 + \log 2 + \log 3 - 2\log 3 + 2\log 2 + \log 3 + \log 2 + 2\log 3 - 2\log 2 - 2\log 3$
   $= 2\log 2 + 2\log 3$

따라서 정답은 **4번: $2\log 2 + 2\log 3$**입니다.

## Question 17
Let $f(n)$ be the number of positive divisors of a natural number $n$, and let $a_1, a_2, a_3, \cdots, a_9$ be all the positive divisors of 36.

What is the value of $\sum_{k=1}^9 \left\{(-1)^{f(a_k)} \times \log a_k\right\}$? **[4 points]**

1. $\log 2 + \log 3$
2. $2\log 2 + \log 3$
3. $\log 2 + 2\log 3$
4. $2\log 2 + 2\log 3$
5. $3\log 2 + 2\log 3$

### Solution
Let's approach this problem step by step:

1. First, list all positive divisors of 36:
   $a_1 = 1, a_2 = 2, a_3 = 3, a_4 = 4, a_5 = 6, a_6 = 9, a_7 = 12, a_8 = 18, a_9 = 36$

2. Calculate $f(a_k)$ for each divisor:
   - $f(1) = 1$
   - $f(2) = 2$
   - $f(3) = 2$
   - $f(4) = 3$
   - $f(6) = 4$
   - $f(9) = 3$
   - $f(12) = 6$
   - $f(18) = 6$
   - $f(36) = 9$

3. Now, let's calculate the given expression:
   $\sum_{k=1}^9 \left\{(-1)^{f(a_k)} \times \log a_k\right\}$
   $= (-1)^1 \log 1 + (-1)^2 \log 2 + (-1)^2 \log 3 + (-1)^3 \log 4 + (-1)^4 \log 6$
   $+ (-1)^3 \log 9 + (-1)^6 \log 12 + (-1)^6 \log 18 + (-1)^9 \log 36$

4. Note that $\log 1 = 0$, so we can ignore the first term. Also, $(-1)$ to an even power is 1, and to an odd power is -1:
   $= \log 2 + \log 3 - \log 4 + \log 6 - \log 9 + \log 12 + \log 18 - \log 36$

5. Using the laws of logarithms, we can simplify:
   $= \log 2 + \log 3 - \log 2^2 + \log (2 \times 3) - \log 3^2 + \log (2^2 \times 3) + \log (2 \times 3^2) - \log (2^2 \times 3^2)$
   $= \log 2 + \log 3 - 2\log 2 + \log 2 + \log 3 - 2\log 3 + 2\log 2 + \log 3 + \log 2 + 2\log 3 - 2\log 2 - 2\log 3$
   $= 2\log 2 + 2\log 3$

Therefore, the correct answer is **4: $2\log 2 + 2\log 3$**.