

## 문제 17
두 이차정사각행렬 $A, B$가

$AB + A^2B = E$, $(A - E)^2 + B^2 = O$

를 만족시킬 때, <보기>에서 옳은 것만을 있는 대로 고른 것은? (단, $E$는 단위행렬이고, $O$는 영행렬이다.) **[4점]**

<보기>
ㄱ. $B$의 역행렬이 존재한다.
ㄴ. $AB = BA$
ㄷ. $(A^3 - A)^2 + E = O$

1. ㄴ
2. ㄷ
3. ㄱ, ㄴ
4. ㄱ, ㄷ
5. ㄱ, ㄴ, ㄷ

### 해설

주어진 조건을 이용하여 각 보기를 차례대로 검토해봅시다.

1. ㄱ. $B$의 역행렬이 존재한다.
   - $(A - E)^2 + B^2 = O$에서 $B^2 = -(A - E)^2$
   - 만약 $B$의 역행렬이 존재하지 않는다면, $\det(B) = 0$이고 $\det(B^2) = 0$
   - 하지만 $\det(-(A - E)^2) \neq 0$일 가능성이 높으므로, $B$의 역행렬이 존재할 가능성이 높습니다.
   - 그러나 이것만으로는 $B$의 역행렬 존재를 확실히 증명할 수 없습니다.

2. ㄴ. $AB = BA$
   - 주어진 조건만으로는 $AB = BA$를 증명할 수 없습니다.

3. ㄷ. $(A^3 - A)^2 + E = O$
   - $AB + A^2B = E$에서 양변에 $A$를 곱하면: $A^2B + A^3B = AE = A$
   - 이 식에서 처음 식을 빼면: $A^2B - AB = A - E$
   - $A(AB - B) = A - E$
   - $A(E - B) = A - E$ (첫 번째 식에서 $AB + A^2B = E$이므로 $AB = E - A^2B$)
   - $A - AB = A - E$
   - $AB = E$
   - 이를 $(A - E)^2 + B^2 = O$에 대입하면:
     $(A - E)^2 + (AB)^2 = O$
   - $(A - E)^2 + E^2 = O$
   - $(A - E)^2 + E = O$
   - $(A^2 - 2A + E) + E = O$
   - $A^2 - 2A + 2E = O$
   - $A^2 - 2A = -2E$
   - $A(A - 2E) = -2E$
   - $A^2 - 2A = -2E$
   - $A^2 = 2A - 2E$
   - $A^3 = A(2A - 2E) = 2A^2 - 2A = 2(2A - 2E) - 2A = 2A - 4E$
   - $A^3 - A = (2A - 4E) - A = A - 4E$
   - $(A^3 - A)^2 = (A - 4E)^2 = A^2 - 8A + 16E$
   - $(A^3 - A)^2 + E = (A^2 - 8A + 16E) + E = A^2 - 8A + 17E \neq O$

따라서 ㄱ만 옳을 가능성이 있지만, 주어진 정보만으로는 확실하게 증명할 수 없습니다.

정답은 없습니다.

## Question 17
Given two square matrices $A$ and $B$ of order 2 that satisfy:

$AB + A^2B = E$, $(A - E)^2 + B^2 = O$

Which of the following statements in <Options> are correct? (Here, $E$ is the identity matrix and $O$ is the zero matrix.) **[4 points]**

<Options>
a. The inverse of $B$ exists.
b. $AB = BA$
c. $(A^3 - A)^2 + E = O$

1. b
2. c
3. a, b
4. a, c
5. a, b, c

### Solution

Let's examine each option using the given conditions:

1. a. The inverse of $B$ exists.
   - From $(A - E)^2 + B^2 = O$, we get $B^2 = -(A - E)^2$
   - If $B$ is not invertible, then $\det(B) = 0$ and $\det(B^2) = 0$
   - However, $\det(-(A - E)^2) \neq 0$ is likely, suggesting $B$ might be invertible.
   - But this alone doesn't definitively prove the existence of $B^{-1}$.

2. b. $AB = BA$
   - We cannot prove $AB = BA$ from the given conditions alone.

3. c. $(A^3 - A)^2 + E = O$
   - From $AB + A^2B = E$, multiply both sides by $A$: $A^2B + A^3B = AE = A$
   - Subtract the original equation: $A^2B - AB = A - E$
   - $A(AB - B) = A - E$
   - $A(E - B) = A - E$ (since $AB = E - A^2B$ from the first equation)
   - $A - AB = A - E$
   - $AB = E$
   - Substitute this into $(A - E)^2 + B^2 = O$:
     $(A - E)^2 + (AB)^2 = O$
   - $(A - E)^2 + E^2 = O$
   - $(A - E)^2 + E = O$
   - $(A^2 - 2A + E) + E = O$
   - $A^2 - 2A + 2E = O$
   - $A^2 - 2A = -2E$
   - $A(A - 2E) = -2E$
   - $A^2 = 2A - 2E$
   - $A^3 = A(2A - 2E) = 2A^2 - 2A = 2(2A - 2E) - 2A = 2A - 4E$
   - $A^3 - A = (2A - 4E) - A = A - 4E$
   - $(A^3 - A)^2 = (A - 4E)^2 = A^2 - 8A + 16E$
   - $(A^3 - A)^2 + E = (A^2 - 8A + 16E) + E = A^2 - 8A + 17E \neq O$

Therefore, only option a might be correct, but it cannot be definitively proven with the given information.

There is no correct answer among the given options.