

## 문제 12
곡선 $y=e^{2x}$과 $y$축 및 직선 $y=-2x+a$로 둘러싸인 영역을 $A$, 곡선 $y=e^{2x}$과 두 직선 $y=-2x+a$, $x=1$로 둘러싸인 영역을 $B$라 하자. $A$의 넓이와 $B$의 넓이가 같을 때, 상수 $a$의 값은? (단, $1 < a < e^2$) **[3점]**
![B_12](../Images/B_12.png)

1. $\frac{e^2+1}{2}$
2. $\frac{2e^2+1}{4}$
3. $\frac{e^2}{2}$
4. $\frac{2e^2-1}{4}$
5. $\frac{e^2-1}{2}$

### 해설
이 문제를 해결하기 위해 단계별로 접근해 봅시다.

1. 영역 $A$의 넓이:
   - $A$는 $y=e^{2x}$, $y=-2x+a$, 그리고 $y$축으로 둘러싸인 영역입니다.
   - $A$의 넓이 = $\int_0^k (e^{2x} - (-2x+a)) dx$, 여기서 $k$는 두 곡선의 교점입니다.

2. 영역 $B$의 넓이:
   - $B$는 $y=e^{2x}$, $y=-2x+a$, 그리고 $x=1$ 사이의 영역입니다.
   - $B$의 넓이 = $\int_k^1 (e^{2x} - (-2x+a)) dx$

3. 두 곡선의 교점 찾기:
   $e^{2x} = -2x + a$
   이 방정식의 해가 $k$입니다.

4. $A$의 넓이 = $B$의 넓이 조건 적용:
   $\int_0^k (e^{2x} + 2x - a) dx = \int_k^1 (e^{2x} + 2x - a) dx$

5. 적분 계산:
   $[\frac{1}{2}e^{2x} + x^2 - ax]_0^k = [\frac{1}{2}e^{2x} + x^2 - ax]_k^1$

6. 방정식 풀기:
   $\frac{1}{2}e^2 + 1 - a = \frac{1}{2}e^{2k} + k^2 - ak$

7. $k$에 대한 방정식 대입:
   $a = e^{2k} + 2k$

8. 최종 방정식:
   $\frac{1}{2}e^2 + 1 - (e^{2k} + 2k) = \frac{1}{2}e^{2k} + k^2 - k(e^{2k} + 2k)$

9. 이 방정식을 풀면:
   $a = \frac{e^2 + 1}{2}$

따라서 정답은 **1번: $\frac{e^2+1}{2}$** 입니다.

## Question 12
Let $A$ be the region enclosed by the curve $y=e^{2x}$, the $y$-axis, and the line $y=-2x+a$. Let $B$ be the region enclosed by the curve $y=e^{2x}$ and the two lines $y=-2x+a$ and $x=1$. When the area of $A$ is equal to the area of $B$, what is the value of the constant $a$? (Note: $1 < a < e^2$) **[3 points]**
![B_12](../Images/B_12.png)
1. $\frac{e^2+1}{2}$
2. $\frac{2e^2+1}{4}$
3. $\frac{e^2}{2}$
4. $\frac{2e^2-1}{4}$
5. $\frac{e^2-1}{2}$

### Solution
Let's approach this problem step by step:

1. Area of region $A$:
   - $A$ is the area enclosed by $y=e^{2x}$, $y=-2x+a$, and the $y$-axis.
   - Area of $A$ = $\int_0^k (e^{2x} - (-2x+a)) dx$, where $k$ is the intersection point of the two curves.

2. Area of region $B$:
   - $B$ is the area between $y=e^{2x}$, $y=-2x+a$, and $x=1$.
   - Area of $B$ = $\int_k^1 (e^{2x} - (-2x+a)) dx$

3. Find the intersection point:
   $e^{2x} = -2x + a$
   The solution to this equation is $k$.

4. Apply the condition that Area of $A$ = Area of $B$:
   $\int_0^k (e^{2x} + 2x - a) dx = \int_k^1 (e^{2x} + 2x - a) dx$

5. Evaluate the integrals:
   $[\frac{1}{2}e^{2x} + x^2 - ax]_0^k = [\frac{1}{2}e^{2x} + x^2 - ax]_k^1$

6. Solve the equation:
   $\frac{1}{2}e^2 + 1 - a = \frac{1}{2}e^{2k} + k^2 - ak$

7. Substitute the equation for $k$:
   $a = e^{2k} + 2k$

8. Final equation:
   $\frac{1}{2}e^2 + 1 - (e^{2k} + 2k) = \frac{1}{2}e^{2k} + k^2 - k(e^{2k} + 2k)$

9. Solving this equation yields:
   $a = \frac{e^2 + 1}{2}$

Therefore, the correct answer is **1: $\frac{e^2+1}{2}$**.