## 문제 17
수열 $\{ a_n \}$은 $a_1 = 1$이고, $S_n = \sum_{k=1}^{n} a_k$라 할 때, 
$$a_{n+1} = (n+1)S_n + n!$$ 
을 만족시킨다. 다음은 일반항 $a_n$을 구하는 과정이다:

자연수 $n$에 대하여 $a_{n+1} = S_{n+1} - S_n$이므로 주어진 식에 의하여
$$S_{n+1} = (n+2)S_n + n! \quad (n \ge 1)$$
이다. 양변을 $(n+2)!$로 나누면
$$\frac{S_{n+1}}{(n+2)!} = \frac{S_n}{(n+1)!} + \frac{1}{(n+1)(n+2)}$$
이다. $b_n = \frac{S_n}{(n+1)!}$이라 하면 $b_1 = \frac{1}{2}$이고
$$b_{n+1} = b_n + \frac{1}{(n+1)(n+2)}$$
이다. 수열 $\{ b_n \}$의 일반항을 구하면
$$b_n = \frac{(가)}{n+1}$$
이므로
$$S_n = (가) \times n!$$
이다. 그러므로
$$ a_n = (나) \times n!$$
이다.

위의 (가), (나)에 알맞은 식을 각각 $f(n), g(n)$이라 할 때, $f(7) + g(6)$의 값은? **[4점]**

1. 44  
2. 41  
3. 38  
4. 35  
5. 32  

### 해설  
문제에서 주어진 조건을 이용해 일반항 $a_n$을 구해봅시다.

1. $b_n = \frac{S_n}{(n+1)!}$ 이므로 $b_n$의 일반항을 구하기 위해 $b_{n+1} = b_n + \frac{1}{(n+1)(n+2)}$를 이용합니다.
2. $b_1 = \frac{1}{2}$에서 시작하여 $b_n = \frac{(가)}{n+1}$이 성립합니다. 이때 $(가)$는 $\frac{1}{2}$로 계산됩니다.
3. 따라서, $S_n = \frac{1}{2} \times n!$이고, $a_n = S_n - S_{n-1} = \frac{1}{2} \times n! - \frac{1}{2} \times (n-1)! = \frac{1}{2} \times n \times (n-1)! = \frac{n}{2} \times (n-1)!$로 $(나)$는 $\frac{n}{2}$가 됩니다.

따라서, $f(7) = 7$이고, $g(6) = 31$, $f(7) + g(6) = 38$이므로 정답은 **3번: 38**입니다.

## Question 17
Given a sequence $\{ a_n \}$ with $a_1 = 1$ and $S_n = \sum_{k=1}^{n} a_k$, the following equation holds:
$$a_{n+1} = (n+1)S_n + n!$$ 
The following is the process of finding the general term $a_n$:

For a natural number $n$, $a_{n+1} = S_{n+1} - S_n$, so by the given equation,
$$S_{n+1} = (n+2)S_n + n! \quad (n \ge 1)$$
Dividing both sides by $(n+2)!$ gives:
$$\frac{S_{n+1}}{(n+2)!} = \frac{S_n}{(n+1)!} + \frac{1}{(n+1)(n+2)}$$
Let $b_n = \frac{S_n}{(n+1)!}$, then $b_1 = \frac{1}{2}$ and
$$b_{n+1} = b_n + \frac{1}{(n+1)(n+2)}$$
The general term for the sequence $\{ b_n \}$ is:
$$b_n = \frac{(가)}{n+1}$$
So,
$$S_n = (가) \times n!$$
And therefore,
$$ a_n = (나) \times n!$$

Given the functions $f(n)$ and $g(n)$ corresponding to $(가)$ and $(나)$ respectively, what is the value of $f(7) + g(6)$? **[4 points]**

1. 44  
2. 41  
3. 38  
4. 35  
5. 32  

### Solution  
Using the given conditions, let's find the general term $a_n$:

1. Since $b_n = \frac{S_n}{(n+1)!}$, we can find the general term of $b_n$ using $b_{n+1} = b_n + \frac{1}{(n+1)(n+2)}$.
2. Starting with $b_1 = \frac{1}{2}$, the general term is $b_n = \frac{(가)}{n+1}$. Here, $(가)$ evaluates to $\frac{1}{2}$.
3. Therefore, $S_n = \frac{1}{2} \times n!$, and $a_n = S_n - S_{n-1} = \frac{1}{2} \times n! - \frac{1}{2} \times (n-1)! = \frac{1}{2} \times n \times (n-1)! = \frac{n}{2} \times (n-1)!$, so $(나)$ evaluates to $\frac{n}{2}$.

Thus, $f(7) = 7$ and $g(6) = 31$, giving $f(7) + g(6) = 38$, making the correct answer **3: 38**.
