## 문제 6
두 일차변환 $f, g$를 나타내는 행렬을 각각 $\begin{pmatrix} 2 & 1 \\ 4 & 2 \end{pmatrix}$, $\begin{pmatrix} 2 & 0 \\ 1 & -1 \end{pmatrix}$이라 하자. 합성변환 $f \circ g$에 의하여 점 $(1, 2)$가 점 $(a, 6)$으로 옮겨질 때, $a$의 값은? **[3점]**

1. 1  
2. 2  
3. 3  
4. 4  
5. 5

### 해설
주어진 문제에서 두 일차변환 $f$와 $g$의 합성변환 $f \circ g$를 사용하여 점 $(1, 2)$가 점 $(a, 6)$으로 이동할 때, $a$의 값을 구하겠습니다.

1. **일차변환 $g$의 계산**:
   먼저, 일차변환 $g$를 점 $(1, 2)$에 적용합니다:
   $$
   g(1, 2) = \begin{pmatrix} 2 & 0 \\ 1 & -1 \end{pmatrix} \begin{pmatrix} 1 \\ 2 \end{pmatrix} = \begin{pmatrix} 2 \times 1 + 0 \times 2 \\ 1 \times 1 + (-1) \times 2 \end{pmatrix} = \begin{pmatrix} 2 \\ -1 \end{pmatrix}
   $$

2. **일차변환 $f$의 계산**:
   이제, 일차변환 $f$를 점 $g(1, 2) = (2, -1)$에 적용합니다:
   $$
   f(2, -1) = \begin{pmatrix} 2 & 1 \\ 4 & 2 \end{pmatrix} \begin{pmatrix} 2 \\ -1 \end{pmatrix} = \begin{pmatrix} 2 \times 2 + 1 \times (-1) \\ 4 \times 2 + 2 \times (-1) \end{pmatrix} = \begin{pmatrix} 4 - 1 \\ 8 - 2 \end{pmatrix} = \begin{pmatrix} 3 \\ 6 \end{pmatrix}
   $$

3. **결과 확인**:
   변환 결과, 점 $(1, 2)$는 점 $(3, 6)$으로 이동합니다. 따라서 $a = 3$입니다.

정답은 **3번: 3**입니다.

---

## Question 6
Let the matrices representing the linear transformations $f$ and $g$ be $\begin{pmatrix} 2 & 1 \\ 4 & 2 \end{pmatrix}$ and $\begin{pmatrix} 2 & 0 \\ 1 & -1 \end{pmatrix}$, respectively. When the point $(1, 2)$ is transformed to $(a, 6)$ by the composite transformation $f \circ g$, what is the value of $a$? **[3 points]**

1. 1  
2. 2  
3. 3  
4. 4  
5. 5

### Solution
Let's find the value of $a$ when the point $(1, 2)$ is transformed by the composite transformation $f \circ g$.

1. **Applying the Transformation $g$**:
   First, apply the transformation $g$ to the point $(1, 2)$:
   $$
   g(1, 2) = \begin{pmatrix} 2 & 0 \\ 1 & -1 \end{pmatrix} \begin{pmatrix} 1 \\ 2 \end{pmatrix} = \begin{pmatrix} 2 \times 1 + 0 \times 2 \\ 1 \times 1 + (-1) \times 2 \end{pmatrix} = \begin{pmatrix} 2 \\ -1 \end{pmatrix}
   $$

2. **Applying the Transformation $f$**:
   Now, apply the transformation $f$ to the point $g(1, 2) = (2, -1)$:
   $$
   f(2, -1) = \begin{pmatrix} 2 & 1 \\ 4 & 2 \end{pmatrix} \begin{pmatrix} 2 \\ -1 \end{pmatrix} = \begin{pmatrix} 2 \times 2 + 1 \times (-1) \\ 4 \times 2 + 2 \times (-1) \end{pmatrix} = \begin{pmatrix} 4 - 1 \\ 8 - 2 \end{pmatrix} = \begin{pmatrix} 3 \\ 6 \end{pmatrix}
   $$

3. **Verify the Result**:
   The point $(1, 2)$ is transformed to the point $(3, 6)$, so $a = 3$.

The correct answer is **3: 3**.
