

## 문제 20. 함수

다음과 같은 함수 $f(x)$가 주어져 있습니다:

$f(x) = \begin{cases}
-x & (x \leq 0) \\
x-1 & (0 < x \leq 2) \\
2x-3 & (x > 2)
\end{cases}$

와 상수가 아닌 다항식 $p(x)$에 대하여 <보기>에서 옳은 것만을 있는 대로 고른 것은? [4점]

<보기>
ㄱ. 함수 $p(x)f(x)$가 실수 전체의 집합에서 연속이면 $p(0) = 0$이다.
ㄴ. 함수 $p(x)f(x)$가 실수 전체의 집합에서 미분가능하면 $p(2) = 0$이다.
ㄷ. 함수 $p(x)(f(x))^2$이 실수 전체의 집합에서 미분가능하면 $p(x)$는 $x^2(x-2)^2$으로 나누어떨어진다.

1. ㄱ
2. ㄱ, ㄴ
3. ㄱ, ㄷ
4. ㄴ, ㄷ
5. ㄱ, ㄴ, ㄷ

### 해설

각 보기를 하나씩 검토해 봅시다.

ㄱ. $p(x)f(x)$가 연속이려면 $x=0$에서 연속이어야 합니다. 
   $\lim_{x \to 0^-} p(x)f(x) = \lim_{x \to 0^-} -xp(x)$
   $\lim_{x \to 0^+} p(x)f(x) = \lim_{x \to 0^+} (x-1)p(x)$
   이 두 극한값이 같아야 하므로, $p(0) \cdot 0 = p(0) \cdot (-1)$
   따라서 $p(0) = 0$이어야 합니다. 옳습니다.

ㄴ. $p(x)f(x)$가 미분가능하려면 $x=2$에서 미분가능해야 합니다.
   왼쪽 극한: $\lim_{h \to 0^-} \frac{p(2+h)f(2+h) - p(2)f(2)}{h} = \lim_{h \to 0^-} \frac{p(2+h)(2+h-1) - p(2)(2-1)}{h}$
   오른쪽 극한: $\lim_{h \to 0^+} \frac{p(2+h)f(2+h) - p(2)f(2)}{h} = \lim_{h \to 0^+} \frac{p(2+h)(2(2+h)-3) - p(2)(2\cdot2-3)}{h}$
   이 두 극한값이 같아야 하므로, $p(2) = 0$이어야 합니다. 옳습니다.

ㄷ. $p(x)(f(x))^2$이 미분가능하려면 $x=0$과 $x=2$에서 미분가능해야 합니다.
   $x=0$에서: $\lim_{x \to 0^-} p(x)x^2 = \lim_{x \to 0^+} p(x)(x-1)^2 = 0$이어야 하므로, $p(x)$는 $x^2$으로 나누어떨어져야 합니다.
   $x=2$에서: $\lim_{x \to 2^-} p(x)(x-1)^2 = \lim_{x \to 2^+} p(x)(2x-3)^2 = 0$이어야 하므로, $p(x)$는 $(x-2)^2$으로 나누어떨어져야 합니다.
   따라서 $p(x)$는 $x^2(x-2)^2$으로 나누어떨어져야 합니다. 옳습니다.

따라서 ㄱ, ㄴ, ㄷ 모두 옳습니다.

정답은 **5번: ㄱ, ㄴ, ㄷ**입니다.

## Question 20. Function

Given the following function $f(x)$:

$f(x) = \begin{cases}
-x & (x \leq 0) \\
x-1 & (0 < x \leq 2) \\
2x-3 & (x > 2)
\end{cases}$

For a non-constant polynomial $p(x)$, which of the following statements in <Options> are correct? [4 points]

<Options>
A. If the function $p(x)f(x)$ is continuous on the set of all real numbers, then $p(0) = 0$.
B. If the function $p(x)f(x)$ is differentiable on the set of all real numbers, then $p(2) = 0$.
C. If the function $p(x)(f(x))^2$ is differentiable on the set of all real numbers, then $p(x)$ is divisible by $x^2(x-2)^2$.

1. A
2. A, B
3. A, C
4. B, C
5. A, B, C

### Solution

Let's examine each statement:

A. For $p(x)f(x)$ to be continuous, it must be continuous at $x=0$. 
   $\lim_{x \to 0^-} p(x)f(x) = \lim_{x \to 0^-} -xp(x)$
   $\lim_{x \to 0^+} p(x)f(x) = \lim_{x \to 0^+} (x-1)p(x)$
   These two limits must be equal, so $p(0) \cdot 0 = p(0) \cdot (-1)$
   Therefore, $p(0) = 0$ must be true. This statement is correct.

B. For $p(x)f(x)$ to be differentiable, it must be differentiable at $x=2$.
   Left limit: $\lim_{h \to 0^-} \frac{p(2+h)f(2+h) - p(2)f(2)}{h} = \lim_{h \to 0^-} \frac{p(2+h)(2+h-1) - p(2)(2-1)}{h}$
   Right limit: $\lim_{h \to 0^+} \frac{p(2+h)f(2+h) - p(2)f(2)}{h} = \lim_{h \to 0^+} \frac{p(2+h)(2(2+h)-3) - p(2)(2\cdot2-3)}{h}$
   These two limits must be equal, so $p(2) = 0$ must be true. This statement is correct.

C. For $p(x)(f(x))^2$ to be differentiable, it must be differentiable at $x=0$ and $x=2$.
   At $x=0$: $\lim_{x \to 0^-} p(x)x^2 = \lim_{x \to 0^+} p(x)(x-1)^2 = 0$ must be true, so $p(x)$ must be divisible by $x^2$.
   At $x=2$: $\lim_{x \to 2^-} p(x)(x-1)^2 = \lim_{x \to 2^+} p(x)(2x-3)^2 = 0$ must be true, so $p(x)$ must be divisible by $(x-2)^2$.
   Therefore, $p(x)$ must be divisible by $x^2(x-2)^2$. This statement is correct.

All statements A, B, and C are correct.

The correct answer is **5: A, B, C**.