We are tasked with finding \( a_9 \) for the sequence \( \{a_n\} \) satisfying the conditions:

1. \( a_1 = a_2 + 3 \)
2. \( a_{n+1} = -2a_n \) for \( n \geq 1 \).

---

### Step 1: Expressing the sequence in terms of \( a_1 \)
The recurrence relation \( a_{n+1} = -2a_n \) gives:
\[
a_2 = -2a_1, \quad a_3 = -2a_2 = -2(-2a_1) = 4a_1, \quad a_4 = -2a_3 = -2(4a_1) = -8a_1,
\]
and so on. The general pattern is:
\[
a_n = (-2)^{n-1} a_1.
\]

---

### Step 2: Using the first condition
The first condition \( a_1 = a_2 + 3 \) becomes:
\[
a_1 = -2a_1 + 3.
\]
Rearranging terms:
\[
a_1 + 2a_1 = 3 \quad \implies \quad 3a_1 = 3 \quad \implies \quad a_1 = 1.
\]

---

### Step 3: Finding \( a_9 \)
Substituting \( a_1 = 1 \) into the general formula \( a_n = (-2)^{n-1} a_1 \):
\[
a_9 = (-2)^{9-1} \cdot 1 = (-2)^8 \cdot 1 = 256.
\]

---

### Final Answer:
\[
\boxed{256}
\]